dimsum_examples/heapUR.v
@@ -2,6 +2,7 @@ From iris.algebra Require Export dfrac.
 From iris.algebra.lib Require Import gmap_view.
 From iris.algebra Require Import agree gset.
 From dimsum.core.iris Require Export biown.
+From dimsum.core.iris Require Import weak_embed.
 From dimsum.examples Require Import rec.
 
 Set Default Proof Using "Type".
@@ -50,7 +51,7 @@ Section heapUR.
 
   Definition heapUR_inv (h : heap_state) : PROP :=
     heapUR_ptsto_auth (h_heap h) ∗
-    heapUR_dom_auth (set_to_map (λ p, (p, dom (h_block h p))) (h_provs h)).
+    heapUR_dom_auth (dom <$> h_blocks h).
 End heapUR.
 
 Notation "l ↦[ O ] dq v" := (heapUR_ptsto O l dq v)
@@ -194,6 +195,15 @@ Section heapUR.
     by apply gmap_view_replace.
   Qed.
 
+  Lemma heapUR_dom_auth_free d p s :
+    heapUR_dom_auth O d ∗ p ↪[O] s ⊢ |==>
+    heapUR_dom_auth O (delete p d).
+  Proof.
+    rewrite -!bi_own_op. rewrite -!pair_op. apply bi_own_bupd.
+    apply prod_update; [done|] => /=. rewrite fmap_delete.
+    by apply gmap_view_delete.
+  Qed.
+
   (** clients should not unfold _inv and only use the lemmas starting from here *)
   Lemma heapUR_uninit_block_eq p dq d `{!BiAffine PROP}:
     heapUR_uninit_block O p dq d ⊣⊢ ∃ b, ⌜d = dom b⌝ ∗ p ↦∗[O]{dq} b.
@@ -239,12 +249,32 @@ Section heapUR.
     iMod (heapUR_ptsto_auth_alloc_big with "Hh") as "[Hh $]". {
       apply map_disjoint_spec => ??? /lookup_kmap_Some[?[->?]] /lookup_heap_Some_elem_of_h_provs. done. }
     iMod (heapUR_dom_auth_alloc with "Hd") as "[Hd $]".
-    { apply eq_None_ne_Some => ?. rewrite lookup_set_to_map; naive_solver. }
+    { rewrite lookup_fmap fmap_None. by apply h_blocks_lookup_None. }
     iModIntro. iFrame. iApply (heapUR_dom_auth_ext with "Hd").
     apply map_eq => p. apply option_eq => ?.
-    rewrite lookup_insert_Some. rewrite !lookup_set_to_map //=.
-    destruct (decide (l.1 = p)); split => ?; destruct!; split!; try set_solver.
-    all: by rewrite ?h_block_heap_alloc // ?h_block_heap_alloc_ne.
+    rewrite lookup_insert_Some !lookup_fmap_Some.
+    setoid_rewrite h_blocks_heap_alloc => //.
+    setoid_rewrite lookup_insert_Some. naive_solver.
+  Qed.
+
+  Lemma heapUR_alloc_loc h l v s Hp:
+    h_heap h !! l = None →
+    heapUR_inv O h -∗
+    l.1 ↪[O] s ==∗
+    heapUR_inv O (heap_alloc_loc h l v Hp) ∗
+    l.1 ↪[O] ({[l.2]} ∪ s) ∗
+    l ↦[O] v.
+  Proof.
+    iIntros (Hl) "[Hh Hd] ?".
+    iMod (heapUR_ptsto_auth_alloc with "Hh") as "[Hh $]"; [done|].
+    iDestruct (heapUR_dom_auth_lookup with "[$] [$]") as %[?[? Hb]]%lookup_fmap_Some.
+    iMod (heapUR_dom_auth_update with "[$]") as "[Hd $]".
+    iModIntro. iFrame. iApply (heapUR_dom_auth_ext with "Hd").
+    apply map_eq => p. apply option_eq => ?.
+    rewrite lookup_insert_Some !lookup_fmap_Some.
+    setoid_rewrite h_blocks_heap_alloc_loc => //.
+    setoid_rewrite lookup_insert_Some.
+    split => ?; destruct!; split!; by rewrite dom_insert_L.
   Qed.
 
   Lemma heapUR_alloc_block h p b:
@@ -256,16 +286,16 @@ Section heapUR.
     iMod (heapUR_ptsto_auth_alloc_big with "Hh") as "[Hh $]". {
       apply map_disjoint_spec => ??? /lookup_kmap_Some[?[->?]] /lookup_heap_Some_elem_of_h_provs. done. }
     iMod (heapUR_dom_auth_alloc with "Hd") as "[Hd $]".
-    { apply eq_None_ne_Some => ?. rewrite lookup_set_to_map; naive_solver. }
+    { rewrite lookup_fmap fmap_None. by apply h_blocks_lookup_None. }
     iModIntro. iSplitL "Hh".
     - iApply (heapUR_ptsto_auth_ext with "Hh") => /=. f_equal.
       apply map_eq => -[??]. apply option_eq => ?. rewrite lookup_kmap_Some lookup_gmap_uncurry bind_Some.
       setoid_rewrite lookup_singleton_Some. naive_solver.
     - iApply (heapUR_dom_auth_ext with "Hd").
       apply map_eq => p2. apply option_eq => ?.
-      rewrite lookup_insert_Some. rewrite !lookup_set_to_map //=.
-      destruct (decide (p = p2)); split => ?; destruct!; split!; try set_solver.
-      all: by rewrite ?h_block_heap_merge_block // ?h_block_heap_merge_block_ne.
+      rewrite lookup_insert_Some !lookup_fmap_Some.
+      setoid_rewrite h_blocks_heap_merge_block => //.
+      setoid_rewrite lookup_insert_Some. naive_solver.
   Qed.
 
   Lemma heapUR_alloc_blocks h bs :
@@ -300,7 +330,7 @@ Section heapUR.
     ⌜dom (h_block h p) = d⌝.
   Proof.
     iIntros "[Hh Hd] Hdom".
-    iDestruct (heapUR_dom_auth_lookup with "[$] [$]") as %[?[? [= ? Hdom]]]%lookup_set_to_map => //.
+    iDestruct (heapUR_dom_auth_lookup with "[$] [$]") as %[?[? [??]%h_blocks_lookup_Some]]%lookup_fmap_Some.
     naive_solver.
   Qed.
 
@@ -310,7 +340,7 @@ Section heapUR.
     ⌜p ∈ h_provs h⌝.
   Proof.
     iIntros "[??] ?".
-    iDestruct (heapUR_dom_auth_lookup with "[$] [$]") as %Hs%lookup_set_to_map => //.
+    iDestruct (heapUR_dom_auth_lookup with "[$] [$]") as %[?[? [??]%h_blocks_lookup_Some]]%lookup_fmap_Some.
     iPureIntro. naive_solver.
   Qed.
 
@@ -321,7 +351,7 @@ Section heapUR.
   Proof.
     iIntros "[Hh Hd] [Hdom Hpts]".
     iDestruct (heapUR_ptsto_auth_lookup_big with "[$] [$]") as %?.
-    iDestruct (heapUR_dom_auth_lookup with "[$] [$]") as %[?[? [= ? Hdom]]]%lookup_set_to_map => //.
+    iDestruct (heapUR_dom_auth_lookup with "[$] [$]") as %[?[Hdom [? ?]%h_blocks_lookup_Some]]%lookup_fmap_Some.
     simplify_eq/=. iPureIntro. apply map_eq => o.
     destruct (b !! o) eqn:Hb.
     - rewrite h_block_lookup. apply: lookup_weaken; [|done].
@@ -346,6 +376,18 @@ Section heapUR.
     ⌜p ∈ h_provs h⌝.
   Proof. iIntros "?[??]". iApply (heapUR_lookup_dom_prov with "[$] [$]"). Qed.
 
+  Lemma heapUR_lookup_block_big h m dq `{!BiPureForall PROP}:
+    heapUR_inv O h -∗
+    ([∗ map] p↦b∈m, p ↦∗[O]{dq} b) -∗
+    ⌜m ⊆ h_blocks h⌝.
+  Proof.
+    iIntros "? Hm". rewrite map_subseteq_spec.
+    iIntros (???). iDestruct (big_sepM_lookup_acc with "[$]") as "[??]"; [done|].
+    iDestruct (heapUR_lookup_block_prov with "[$] [$]") as %?.
+    iDestruct (heapUR_lookup_block with "[$] [$]") as %?. subst.
+    iPureIntro. by apply h_blocks_lookup_Some.
+  Qed.
+
   Lemma heapUR_update v' h l v:
     heapUR_inv O h -∗
     l ↦[O] v ==∗
@@ -358,12 +400,14 @@ Section heapUR.
     - iApply (heapUR_ptsto_auth_ext with "[$]"). apply partial_alter_ext.
       move => ??. by simplify_map_eq.
     - iApply (heapUR_dom_auth_ext with "[$]").
-      apply map_eq => ?. apply option_eq => ?.
-      rewrite !lookup_set_to_map //=. f_equiv => ?. do 3 f_equiv. apply set_eq => ?.
-      by rewrite !elem_of_dom !h_block_lookup/= lookup_alter_is_Some.
+      rewrite h_blocks_heap_update.
+      apply map_eq => p. apply option_eq => ?.
+      rewrite !lookup_fmap_Some.
+      setoid_rewrite lookup_alter_Some.
+      destruct (decide (p = l.1)); split => ?; destruct!; split!; by rewrite dom_alter_L.
   Qed.
 
-  Lemma heapUR_update_block v' h l b:
+  Lemma heapUR_update_in_block v' h l b:
     heap_alive h l →
     heapUR_inv O h -∗
     l.1 ↦∗[O] b ==∗
@@ -379,6 +423,25 @@ Section heapUR.
     iSplitL "Hdom".
     - rewrite dom_insert_lookup_L //. eexists _. by rewrite -h_block_lookup2.
     - rewrite kmap_insert. by iApply "Hl".
+  Qed.
+
+  Lemma heapUR_update_block b' h p b:
+    heapUR_inv O h -∗
+    p ↦∗[O] b ==∗
+    heapUR_inv O (heap_update_block h p b') ∗ p ↦∗[O] b'.
+  Proof.
+    iIntros "Hinv Hb".
+    iDestruct (heapUR_lookup_block with "[$] [$]") as %<-.
+    iDestruct "Hinv" as "[Hh Hd]". iDestruct "Hb" as "[Hdom Hpts]".
+    iMod (heapUR_ptsto_auth_free_big with "Hh Hpts") as "Hh".
+    rewrite h_heap_difference_block.
+    iMod (heapUR_dom_auth_update with "[$]") as "[Hdom $]".
+    iMod (heapUR_ptsto_auth_alloc_big with "Hh") as "[Hh $]". {
+      apply map_disjoint_spec => ???/lookup_kmap_Some[?[??]].
+      move => /map_lookup_filter_Some. naive_solver.
+    }
+    iModIntro. iFrame.
+    by rewrite h_blocks_heap_update_block fmap_insert.
   Qed.
 
   Lemma heapUR_free l h b:
@@ -400,14 +463,8 @@ Section heapUR.
       move => [Hh Hi]. split; [done|]. move => Heq.
       rewrite h_block_lookup2 Heq Hi // in Hh. by rewrite -Heq -surjective_pairing.
     - iApply (heapUR_dom_auth_ext with "[$]").
-      rewrite h_provs_heap_free //.
-      apply map_eq => p. apply option_eq => ?.
-      rewrite lookup_insert_Some !lookup_set_to_map //=.
-      destruct (decide (l.1 = p)); split => ?; destruct!; split!.
-      + by rewrite h_block_free.
-      + by rewrite h_block_free.
-      + by rewrite h_block_free_ne.
-      + by rewrite h_block_free_ne.
+      rewrite h_blocks_free -fmap_insert alter_eq_insert_const //.
+      by apply h_blocks_lookup_is_Some.
   Qed.
 
   Lemma heapUR_free_uninit l h b `{!BiAffine PROP}:
@@ -418,6 +475,46 @@ Section heapUR.
     iIntros "Hinv Hb".
     iDestruct (heapUR_uninit_block_eq with "Hb") as (? ->) "?".
     by iApply (heapUR_free with "[$]").
+  Qed.
+
+  Lemma heapUR_remove_prov p h b:
+    heapUR_inv O h -∗
+    p ↦∗[O] b ==∗
+    heapUR_inv O (heap_remove_prov h p).
+  Proof.
+    iIntros "Hinv Hb".
+    iDestruct (heapUR_lookup_block with "[$] [$]") as %<-.
+    iDestruct (heapUR_lookup_block_prov with "[$] [$]") as %?.
+    iDestruct "Hinv" as "[Hh Hd]". iDestruct "Hb" as "[Hdom Hpts]".
+    iMod (heapUR_ptsto_auth_free_big with "Hh Hpts") as "Hh".
+    iMod (heapUR_dom_auth_free with "[$]") as "?". iModIntro.
+    iSplitL "Hh".
+    - iApply (heapUR_ptsto_auth_ext with "[$]") => /=. by rewrite h_heap_difference_block.
+    - iApply (heapUR_dom_auth_ext with "[$]").
+      apply map_eq => p'. apply option_eq => ?.
+      rewrite lookup_delete_Some !lookup_fmap_Some.
+      setoid_rewrite h_blocks_heap_remove_prov.
+      setoid_rewrite lookup_delete_Some.
+      naive_solver.
+  Qed.
+
+  Lemma heapUR_remove_loc h l v s:
+    heapUR_inv O h -∗
+    l ↦[O] v -∗
+    l.1 ↪[O] s ==∗
+    heapUR_inv O (heap_remove_loc h l) ∗
+    l.1 ↪[O] (s ∖ {[l.2]}).
+  Proof.
+    iIntros "[Hh Hd] ? ?".
+    iMod (heapUR_ptsto_auth_free with "[$]") as "Hh".
+    iDestruct (heapUR_dom_auth_lookup with "[$] [$]") as %[?[? ?]]%lookup_fmap_Some.
+    iMod (heapUR_dom_auth_update with "[$]") as "[Hd $]".
+    iModIntro. iFrame. iApply (heapUR_dom_auth_ext with "Hd").
+    apply map_eq => p. apply option_eq => ?.
+    rewrite lookup_insert_Some !lookup_fmap_Some.
+    setoid_rewrite h_blocks_heap_remove_loc => //.
+    setoid_rewrite lookup_insert_Some.
+    split => ?; destruct!; split!; by rewrite dom_delete_L.
   Qed.
 
   (** init *)
@@ -433,7 +530,7 @@ Section heapUR.
   Proof.
     have ? := bi_own_proper _ _ O. rewrite /heapUR_init pair_split bi_own_op.
     iIntros "[$ Ho]" => /=. iApply (heapUR_dom_auth_ext with "Ho").
-    apply map_eq => ?. apply option_eq => ?. by rewrite lookup_set_to_map.
+    apply map_eq => ?. apply option_eq => ?. by rewrite lookup_fmap_Some.
   Qed.
 
 End heapUR.
@@ -441,3 +538,492 @@ End heapUR.
 Global Typeclasses Opaque heapUR_ptsto heapUR_dom heapUR_inv.
 Global Opaque heapUR_ptsto heapUR_dom heapUR_inv.
 Global Arguments heapUR_block : simpl never.
+
+(** * Trader for HeapUR *)
+(* TODO: Better name? Trade Post? Warp Gate? *)
+
+Section trader.
+  Context {PROP1 PROP2 PROP : bi} `{!BiBUpd PROP1} `{!BiBUpd PROP2}.
+  Context (W1 : BiWeakEmbed PROP1 PROP) (W2 : BiWeakEmbed PROP2 PROP).
+  Context (O1 : BiOwn PROP1 heapUR) (O2 : BiOwn PROP2 heapUR).
+
+  Definition heapUR_ptsto_trader (l : loc) (v : val) : PROP :=
+    ⌈l ↦[O1] v @ W1⌉ ∨ ⌈l ↦[O2] v @ W2⌉.
+  Definition heapUR_dom_trader (p : prov) (d : gset Z) : PROP :=
+    ⌈p ↪[O1] d @ W1⌉ ∨ ⌈p ↪[O2] d @ W2⌉.
+  Definition heapUR_block_trader (p : prov) (b : gmap Z val) : PROP :=
+    heapUR_dom_trader p (dom b) ∗
+    ([∗ map] l↦v∈kmap (pair p) b, heapUR_ptsto_trader l v).
+  Definition heapUR_heap_trader (h : heap_state) : PROP :=
+    ⌈heapUR_inv O1 h @ W1⌉ ∗
+    ([∗ map] p↦b∈h_blocks h, heapUR_block_trader p b).
+
+  Definition heapUR_trader : PROP := ∃ h, heapUR_heap_trader h.
+
+  Context `{!BiBUpd PROP} `{!BiAffine PROP} `{!BiWeakEmbedBUpd W1} `{!BiWeakEmbedBUpd W2}.
+
+  Lemma heapUR_block_trader_or p b :
+    ⌈p ↦∗[O1] b @ W1⌉ ∨ ⌈p ↦∗[O2] b @ W2⌉ ⊢ heapUR_block_trader p b.
+  Proof using BiAffine0.
+    rewrite /heapUR_block_trader.
+    iIntros "[[Hd ?]|[Hd ?]]"; (iSplitL "Hd"; [(by iLeft) || by iRight|]).
+    all: rewrite weak_embed_big_sepM.
+    all: iApply (big_sepM_impl with "[$]").
+    all: iIntros "!>" (???) "?".
+    - by iLeft.
+    - by iRight.
+  Qed.
+
+  Global Instance from_or_heapUR_block_trader p b :
+    FromOr (heapUR_block_trader p b) ⌈p ↦∗[O1] b @ W1⌉ ⌈p ↦∗[O2] b @ W2⌉.
+  Proof using BiAffine0. by rewrite /FromOr heapUR_block_trader_or. Qed.
+
+  Lemma heapUR_ptsto_trader_in_1 h2 l v :
+    h_heap h2 !! l = None →
+    ⌈heapUR_inv O2 h2 @ W2⌉ -∗
+    heapUR_ptsto_trader l v -∗
+    ⌈l ↦[O1] v @ W1⌉ ∗ ⌈heapUR_inv O2 h2 @ W2⌉.
+  Proof using BiAffine0.
+    iIntros (?) "? [$|?]" => //.
+    iDestruct (heapUR_lookup O2 with "[$] [$]") as %?.
+    naive_solver.
+  Qed.
+
+  Lemma heapUR_dom_trader_in_1 h2 p d :
+    p ∉ h_provs h2 ∨ d ≠ dom (h_block h2 p) →
+    ⌈heapUR_inv O2 h2 @ W2⌉ -∗
+    heapUR_dom_trader p d -∗
+    ⌈p ↪[O1] d @ W1⌉ ∗ ⌈heapUR_inv O2 h2 @ W2⌉.
+  Proof using BiAffine0.
+    iIntros (?) "? [$|?]" => //.
+    iDestruct (heapUR_lookup_dom O2 with "[$] [$]") as %?.
+    iDestruct (heapUR_lookup_dom_prov O2 with "[$] [$]") as %?.
+    naive_solver.
+  Qed.
+
+  Lemma heapUR_block_trader_in_1 h2 p bs :
+    p ∉ h_provs h2 →
+    ⌈heapUR_inv O2 h2 @ W2⌉ -∗
+    heapUR_block_trader p bs -∗
+    ⌈p ↦∗[O1] bs @ W1⌉ ∗ ⌈heapUR_inv O2 h2 @ W2⌉.
+  Proof using BiAffine0.
+    iIntros (?) "? [??]".
+    iDestruct (heapUR_dom_trader_in_1 with "[$] [$]") as "[$ ?]". 1: naive_solver.
+    rewrite weak_embed_big_sepM.
+    iApply (big_sepM_impl_frame with "[$]"). 2: done.
+    iIntros "!>" (?? Hk) "??". iDestruct (heapUR_ptsto_trader_in_1 with "[$] [$]") as "[$ $]".
+    apply not_elem_of_h_provs_lookup_heap. move: Hk => /lookup_kmap_Some. naive_solver.
+  Qed.
+
+
+  Lemma heapUR_heap_trader_equalize h1 h2 :
+    heapUR_heap_trader h1 -∗
+    ⌈heapUR_inv O2 h2 @ W2⌉ ==∗⌈W1⌉
+    heapUR_heap_trader h2 ∗
+    ⌈heapUR_inv O2 h2 @ W2⌉.
+  Proof using BiWeakEmbedBUpd1 BiWeakEmbedBUpd0 BiAffine0.
+    iIntros "(Hinv1 & Hb) Hinv2".
+    have [bs Hbs] : ∃ bs, bs = h_blocks h1 by naive_solver.
+    iInduction bs as [p bs ? Hp1 Hp2|p bs ? Hp1 Hp2|p bs1 bs2 ? Hp1 Hp2|] "IH" using (map_equalize_ind (h_blocks h2)) forall (h1 Hbs); subst.
+    - move: Hp1 => /h_blocks_lookup_None ?.
+      iMod (heapUR_alloc_block O1 _ p bs with "Hinv1") as "[? Hbs]"; [done|].
+      iApply ("IH" with "[%] [$] [Hb Hbs] [$]").
+      + rewrite h_blocks_heap_merge /= ?dom_singleton_L; [|set_solver].
+        by rewrite h_blocks_heap_from_blocks insert_union_singleton_l.
+      + rewrite h_blocks_heap_merge /= ?dom_singleton_L; [|set_solver].
+        rewrite h_blocks_heap_from_blocks -insert_union_singleton_l.
+        iApply (big_sepM_insert_2 with "[Hbs] Hb"). by iLeft.
+    - iDestruct (big_sepM_delete with "Hb") as "[? Hm]"; [done|].
+      iDestruct (heapUR_block_trader_in_1 with "[$] [$]") as "[? ?]".
+      { by apply h_blocks_lookup_None. }
+      iMod (heapUR_remove_prov O1 with "[$] [$]").
+      by iApply ("IH" with "[%] [$] [Hm] [$]"); rewrite h_blocks_heap_remove_prov.
+    - iInduction bs1 as [o v ? Hb1 Hb2|o v ? Hb1 Hb2|o v1 v2|] "IH2" using (map_equalize_ind bs2) forall (h1 Hp1) "IH".
+      + iDestruct (big_sepM_insert_acc with "Hb") as "[[Hd Hls] Hc]"; [done|].
+        iDestruct (heapUR_dom_trader_in_1 with "[$] [$]") as "[??]". {
+          right. move => Hd. move: Hp1 => /h_blocks_lookup_Some[??].
+          move: Hp2 => /h_blocks_lookup_Some[??]. subst.
+          move: Hb1 => /not_elem_of_dom. rewrite Hd => /not_elem_of_dom.
+          naive_solver.
+        }
+        iDestruct (heapUR_lookup_dom_prov O1 with "Hinv1 [$]") as %Hp.
+        iMod (heapUR_alloc_loc O1 _ (p, o) _ _ Hp with "[$] [$]") as "[? [Hp Hl]]" => /=.
+        { rewrite -h_block_lookup. by move: Hp1 => /h_blocks_lookup_Some[? <-]. }
+        erewrite <-dom_insert_L.
+        iDestruct ("Hc" with "[$Hp Hl Hls]") as "Hb".
+        { rewrite kmap_insert. iApply (big_sepM_insert_2 with "[Hl] [$]"). by iLeft. }
+        iApply ("IH2" with "[%] [$] [Hb] [$]").
+        * erewrite h_blocks_heap_alloc_loc => //=. by simplify_map_eq.
+        * erewrite h_blocks_heap_alloc_loc => //=.
+        * iIntros "!>" (? Heq). iApply "IH". iPureIntro. rewrite -Heq.
+          erewrite h_blocks_heap_alloc_loc => //=. by rewrite insert_insert.
+      + iDestruct (big_sepM_insert_acc with "Hb") as "[[Hd Hls] Hc]"; [done|].
+        iDestruct (heapUR_dom_trader_in_1 with "[$] [$]") as "[??]". {
+          right. move => Hd. move: Hp1 => /h_blocks_lookup_Some[??].
+          move: Hp2 => /h_blocks_lookup_Some[??]. subst.
+          move: Hb2 => /not_elem_of_dom. rewrite -Hd => /not_elem_of_dom.
+          naive_solver.
+        }
+        iDestruct (big_sepM_delete with "Hls") as "[? Hls]".
+        { apply/lookup_kmap_Some. naive_solver. }
+        iDestruct (heapUR_ptsto_trader_in_1 with "[$] [$]") as "[??]".
+        { rewrite -h_block_lookup. by move: Hp2 => /h_blocks_lookup_Some[? <-]. }
+        iMod (heapUR_remove_loc O1 with "[$] [$] [$]") as "[? Hp]" => /=.
+        erewrite <-dom_delete_L. rewrite -kmap_delete.
+        iDestruct ("Hc" with "[$Hp $Hls]") as "Hb".
+        iApply ("IH2" with "[%] [$] [Hb] [$]").
+        * erewrite h_blocks_heap_remove_loc => //=. by simplify_map_eq.
+        * erewrite h_blocks_heap_remove_loc => //=.
+        * iIntros "!>" (? Heq). iApply "IH". iPureIntro. rewrite -Heq.
+          erewrite h_blocks_heap_remove_loc => //=. by rewrite insert_insert.
+      + iDestruct (big_sepM_insert_acc with "Hb") as "[[Hd Hls] Hc]"; [done|].
+        iDestruct (big_sepM_insert_acc with "Hls") as "[Ht Hc2]".
+        { apply/lookup_kmap_Some. naive_solver. }
+        iDestruct "Ht" as "[Ht|Ht]".
+        * iMod (heapUR_update O1 with "[$] [$]") as "[? Hl]".
+          iDestruct ("Hc2" with "[Hl]") as "Hb"; [by iLeft|]. rewrite -kmap_insert.
+          iDestruct ("Hc" with "[$Hb Hd]") as "Hb". { by rewrite dom_insert_lookup_L. }
+          iApply ("IH2" with "[%] [$] [Hb] [$]").
+          -- rewrite h_blocks_heap_update /= lookup_alter Hp1 /= alter_eq_insert_const //.
+          -- rewrite h_blocks_heap_update /=. erewrite (alter_eq_insert (h_blocks h1)) => //.
+             rewrite alter_eq_insert_const //.
+          -- iIntros "!>" (? Heq). iApply "IH". iPureIntro. rewrite -Heq.
+             by rewrite h_blocks_heap_update /= insert_alter.
+        * iDestruct (heapUR_lookup O2 with "[$] [$]") as %Hpo.
+          have ? : v2 = v1. {
+            move: Hp2 => /h_blocks_lookup_Some[??]. move: Hpo. rewrite -h_block_lookup. naive_solver.
+          } subst.
+          iDestruct ("Hc2" with "[Ht]") as "Hb"; [by iRight|].
+          rewrite -kmap_insert insert_id //.
+          iDestruct ("Hc" with "[$Hb $Hd]") as "Hb". rewrite (insert_id _ p bs1) //.
+          iApply ("IH2" with "[//] [$] [$] [$] [$]").
+      + iApply ("IH" with "[%] [$] [$] [$]"). by rewrite insert_id.
+    - move: Hbs => /heap_state_blocks_eq ->. by iFrame.
+  Qed.
+
+  Lemma heapUR_ptsto_trader_trade l v :
+    ⌈l ↦[O2] v @ W2⌉ -∗
+    heapUR_ptsto_trader l v -∗
+    heapUR_ptsto_trader l v ∗
+    ⌈l ↦[O1] v @ W1⌉.
+  Proof using BiAffine0.
+    iIntros "Hl [?|?]".
+    - by iFrame "Hl".
+    - iDestruct (heapUR_ptsto_excl O2 with "[$] [$]") as %[].
+  Qed.
+
+  Lemma heapUR_dom_trader_trade p d :
+    ⌈p ↪[O2] d @ W2⌉ -∗
+    heapUR_dom_trader p d -∗
+    heapUR_dom_trader p d ∗
+    ⌈p ↪[O1] d @ W1⌉.
+  Proof using BiAffine0.
+    iIntros "Hl [?|?]".
+    - by iFrame "Hl".
+    - iDestruct (heapUR_dom_excl O2 with "[$] [$]") as %[].
+  Qed.
+
+
+  (** Trader lemmas  *)
+  Lemma heapUR_trader_init_blocks hinit :
+    ⌈heapUR_inv O1 (heap_from_blocks hinit) @ W1⌉ -∗
+    ⌈[∗ map] p↦b∈hinit, p↦∗[O2] b @ W2⌉ -∗
+    heapUR_trader.
+  Proof using BiAffine0.
+    iIntros "? Hinit". iFrame.
+    rewrite !weak_embed_big_sepM h_blocks_heap_from_blocks.
+    iApply (big_sepM_impl with "Hinit"). iIntros "!>" (???) "?". by iRight.
+  Qed.
+
+  Lemma heapUR_trade_ptsto h l v:
+    heapUR_trader -∗
+    ⌈heapUR_inv O2 h @ W2⌉ -∗
+    ⌈l ↦[O2] v @ W2⌉ ==∗⌈W1⌉
+    heapUR_trader ∗
+    ⌈heapUR_inv O2 h @ W2⌉ ∗
+    ⌈l ↦[O1] v @ W1⌉.
+  Proof using BiWeakEmbedBUpd1 BiWeakEmbedBUpd0 BiAffine0.
+    iIntros "[%h1 Hinv1] Hinv2 Hl".
+    iMod (heapUR_heap_trader_equalize with "Hinv1 [$]") as "[[Hinv1 Hbs] Hinv2]".
+    iDestruct (heapUR_lookup O2 with "[$] Hl") as %?.
+    iDestruct (big_sepM_lookup_acc with "Hbs") as "[[Hd Hls] Hc]".
+    { apply h_blocks_lookup_Some. split!. by apply: lookup_heap_Some_elem_of_h_provs. }
+    iDestruct (big_sepM_lookup_acc with "Hls") as "[Hp Hc2]".
+    { apply/lookup_kmap_Some. eexists l.2. split!. by rewrite -h_block_lookup2. }
+    rewrite -surjective_pairing.
+    iDestruct (heapUR_ptsto_trader_trade with "[$] [$]") as "[? $]".
+    iDestruct ("Hc2" with "[$]") as "?".
+    iDestruct ("Hc" with "[$]") as "?".
+    by iFrame.
+  Qed.
+
+  Lemma heapUR_trade_dom h p d:
+    heapUR_trader -∗
+    ⌈heapUR_inv O2 h @ W2⌉ -∗
+    ⌈p ↪[O2] d @ W2⌉ ==∗⌈W1⌉
+    heapUR_trader ∗
+    ⌈heapUR_inv O2 h @ W2⌉ ∗
+    ⌈p ↪[O1] d @ W1⌉.
+  Proof using BiWeakEmbedBUpd1 BiWeakEmbedBUpd0 BiAffine0.
+    iIntros "[%h1 Hinv1] Hinv2 Hl".
+    iMod (heapUR_heap_trader_equalize with "Hinv1 [$]") as "[[Hinv1 Hbs] Hinv2]".
+    iDestruct (heapUR_lookup_dom O2 with "[$] Hl") as %<-.
+    iDestruct (heapUR_lookup_dom_prov O2 with "[$] Hl") as %?.
+    iDestruct (big_sepM_lookup_acc with "Hbs") as "[[Hd Hls] Hc]".
+    { by apply h_blocks_lookup_Some. }
+    iDestruct (heapUR_dom_trader_trade with "[$] [$]") as "[? $]".
+    iDestruct ("Hc" with "[$]") as "?".
+    by iFrame.
+  Qed.
+
+  Lemma heapUR_trade_ptsto_big h m:
+    heapUR_trader -∗
+    ⌈heapUR_inv O2 h @ W2⌉ -∗
+    ⌈[∗ map] l↦v∈m, l ↦[O2] v @ W2⌉ ==∗⌈W1⌉
+    heapUR_trader ∗
+    ⌈heapUR_inv O2 h @ W2⌉ ∗
+    ⌈[∗ map] l↦v∈m, l ↦[O1] v @ W1⌉.
+  Proof using BiWeakEmbedBUpd1 BiWeakEmbedBUpd0 BiAffine0.
+    iIntros "Ht Hinv Hl".
+    iInduction m as [|] "IH" using map_ind.
+    { iModIntro. iFrame. iModIntro. done. }
+    rewrite !big_sepM_insert //. iDestruct "Hl" as "[??]".
+    iMod (heapUR_trade_ptsto with "[$] [$] [$]") as "[? [? $]]".
+    iApply ("IH" with "[$] [$] [$]").
+  Qed.
+
+  Lemma heapUR_trade_block h p b:
+    heapUR_trader -∗
+    ⌈heapUR_inv O2 h @ W2⌉ -∗
+    ⌈p ↦∗[O2] b @ W2⌉ ==∗⌈W1⌉
+    heapUR_trader ∗
+    ⌈heapUR_inv O2 h @ W2⌉ ∗
+    ⌈p ↦∗[O1] b @ W1⌉.
+  Proof using BiWeakEmbedBUpd1 BiWeakEmbedBUpd0 BiAffine0.
+    iIntros "Ht Hinv [Hd Hl]".
+    iMod (heapUR_trade_dom with "[$] [$] [$]") as "[? [? $]]".
+    by iMod (heapUR_trade_ptsto_big with "[$] [$] [$]") as "$".
+  Qed.
+
+  Lemma heapUR_trade_block_big h bs:
+    heapUR_trader -∗
+    ⌈heapUR_inv O2 h @ W2⌉ -∗
+    ⌈[∗ map] p↦b∈ bs, p ↦∗[O2] b @ W2⌉ ==∗⌈W1⌉
+    heapUR_trader ∗
+    ⌈heapUR_inv O2 h @ W2⌉ ∗
+    ⌈[∗ map] p↦b∈ bs, p ↦∗[O1] b @ W1⌉.
+  Proof using BiWeakEmbedBUpd1 BiWeakEmbedBUpd0 BiAffine0.
+    iIntros "Ht Hinv Hbs".
+    rewrite !weak_embed_big_sepM.
+    iMod (big_sepM_impl_weak_bupd_frame with "Hbs [] [-]") as "[$ ?]". 2: iAccu. 2: by iModIntro.
+    iIntros "!>" (???) "[??] ?".
+    by iMod (heapUR_trade_block with "[$] [$] [$]") as "[$ [$ $]]".
+  Qed.
+End trader.
+
+Section trader.
+  Context {PROP1 PROP2 PROP : bi} `{!BiBUpd PROP1} `{!BiBUpd PROP2}.
+  Context (W1 : BiWeakEmbed PROP1 PROP) (W2 : BiWeakEmbed PROP2 PROP).
+  Context (O1 : BiOwn PROP1 heapUR) (O2 : BiOwn PROP2 heapUR).
+  Context `{!BiBUpd PROP} `{!BiAffine PROP} `{!BiWeakEmbedBUpd W1} `{!BiWeakEmbedBUpd W2}.
+
+  Lemma heapUR_ptsto_trader_switch l v :
+    heapUR_ptsto_trader W1 W2 O1 O2 l v -∗
+    heapUR_ptsto_trader W2 W1 O2 O1 l v.
+  Proof using BiAffine0. iIntros "[$|$]". Qed.
+
+  Lemma heapUR_dom_trader_switch p d :
+    heapUR_dom_trader W1 W2 O1 O2 p d -∗
+    heapUR_dom_trader W2 W1 O2 O1 p d.
+  Proof using BiAffine0. iIntros "[$|$]". Qed.
+
+  Lemma heapUR_block_trader_switch p b :
+    heapUR_block_trader W1 W2 O1 O2 p b -∗
+    heapUR_block_trader W2 W1 O2 O1 p b.
+  Proof using BiAffine0.
+    iIntros "[??]".
+    iDestruct (heapUR_dom_trader_switch with "[$]") as "$".
+    iApply (big_sepM_impl with "[$]"). iIntros "!>" (???) "?".
+    by iApply heapUR_ptsto_trader_switch.
+  Qed.
+
+  (** Trader lemmas  *)
+  Lemma heapUR_trader_switch h :
+    heapUR_trader W1 W2 O1 O2 -∗
+    ⌈heapUR_inv O2 h @ W2⌉ ==∗⌈W1⌉
+    heapUR_trader W2 W1 O2 O1 ∗
+    ⌈heapUR_inv O1 h @ W1⌉.
+  Proof using BiWeakEmbedBUpd1 BiWeakEmbedBUpd0 BiAffine0.
+    iIntros "[%h1 Hinv1] Hinv2".
+    iMod (heapUR_heap_trader_equalize with "Hinv1 [$]") as "[[??] ?]".
+    iModIntro. iFrame. iApply (big_sepM_impl with "[$]").
+    iIntros "!>" (???) "?". by iApply heapUR_block_trader_switch.
+  Qed.
+
+End trader.
+
+(*
+Section trader.
+  Context {PROP1 PROP2 PROP : bi}.
+  Context `{!BiBUpd PROP1} `{!BiBUpd PROP2} `{!BiBUpd PROP} `{!BiAffine PROP}.
+  Context (W1 : BiWeakEmbed PROP1 PROP) (W2 : BiWeakEmbed PROP2 PROP).
+  Context `{!BiWeakEmbedBUpd W1} `{!BiWeakEmbedBUpd W2}.
+  Context (O1 : BiOwn PROP1 heapUR) (O2 : BiOwn PROP2 heapUR).
+
+  Lemma heapUR_trader_init_blocks hinit :
+    ⌈heapUR_inv O2 (heap_from_blocks hinit) @ W2⌉ -∗
+    ⌈[∗ map] p↦b∈hinit, p↦∗[O1] b @ W1⌉ -∗
+    heapUR_trader W2 W1 O2 O1.
+  Proof.
+    iIntros "? Hinit". iFrame. unfold heapUR_block. rewrite big_sepM_sep.
+    iDestruct "Hinit" as "[??]".
+    rewrite !weak_embed_big_sepM. iExists ∅, ∅.
+  Abort.
+
+
+  Lemma heapUR_trader_switch h :
+    heapUR_trader W1 W2 O1 O2 -∗
+    ⌈heapUR_inv O2 h @ W2⌉ ==∗⌈W1⌉
+    heapUR_trader W2 W1 O2 O1 ∗
+    ⌈heapUR_inv O1 h @ W1⌉.
+  Proof.
+    iIntros "(%h1 & %ls & %ds & Hinv1 & Hls1 & Hds1 & Hls2 & Hds2) Hinv".
+    have [ps Hps] : ∃ ps, ps = h_provs h1 by naive_solver.
+    iInduction ps as [p ps| p ps |] "IH" using (set_equalize_ind_L (h_provs h)) forall (h1 ls ds Hps); subst.
+    - iMod (heapUR_alloc_block O1 _ p ∅ with "Hinv1") as "[? [Hd _]]"; [done|].
+      iApply ("IH" with "[%] [$] [$] [Hd Hds1] [Hls2] [Hds2] [$]").
+      + by rewrite /= dom_singleton_L.
+      + by iApply (big_sepM_insert_2 with "[Hd] Hds1").
+      + simpl. admit.
+      + admit.
+    - admit.
+    -
+
+admit.
+    (* add new provenances to h1 *)
+    (* delete removed provenances from h1 *)
+    (* update all heap locations to match *)
+  Abort.
+
+  Lemma heapUR_trade_ptsto h l v:
+    heapUR_trader W1 W2 O1 O2 -∗
+    (* TODO: Do we need this? *)
+    ⌈heapUR_inv O2 h @ W2⌉ -∗
+    ⌈l ↦[O2] v @ W2⌉ ==∗⌈W1⌉
+    heapUR_trader W1 W2 O1 O2 ∗
+    ⌈heapUR_inv O2 h @ W2⌉ ∗
+    ⌈l ↦[O1] v @ W1⌉.
+  Proof.
+    iIntros "(%h1 & %ls & %ds & Hinv1 & Hls1 & Hds1 & Hls2 & Hds2) Hinv Hl".
+    (* TODO: Is there a better way to prove this via heapUR_trader_switch? *)
+    destruct (h_heap h1 !! l) eqn:Hh1.
+    - destruct (ls !! l) eqn: Hls.
+      + iDestruct (big_sepM_delete with "Hls1") as "[Hl' Hls1]"; [done|].
+        (* Set Typeclasses Debug Verbosity 2. *)
+        iMod (heapUR_update O1 with "[$] [$]") as "[??]".
+        iModIntro. iFrame. rewrite h_block_doms_h_update. iFrame => /=.
+        erewrite difference_delete. 2: { apply lookup_alter_Some. naive_solver. }
+        rewrite insert_difference insert_alter -insert_difference.
+        by iApply (big_sepM_insert_2 with "[Hl]").
+      + iDestruct (big_sepM_lookup_acc _ _ l with "Hls2") as "[??]".
+        { by apply lookup_difference_Some. }
+        iDestruct (heapUR_ptsto_excl (PROP:=PROP2) with "Hl [$]") as %[].
+    - destruct (decide (l.1 ∈ h_provs h1)).
+      + destruct (ds !! l.1) eqn:Hds.
+        * (* get heapUR_dom O1 l.1 g, update h1 to add l to the heap, return ownership    *)
+          admit.
+        * iDestruct (big_sepM_lookup_acc with "Hds2") as "[Hd ?]".
+          { apply lookup_difference_Some. split; [|done]. by apply h_block_doms_lookup_Some. }
+          iDestruct (heapUR_lookup (PROP:=PROP2) with "Hinv Hl") as %?.
+          iDestruct (heapUR_lookup_dom (PROP:=PROP2) with "Hinv Hd") as %Heq.
+          exfalso. have : l.2 ∈ dom (h_block h l.1).
+          -- apply elem_of_dom. by rewrite -h_block_lookup2.
+          -- rewrite Heq => /elem_of_dom. by rewrite -h_block_lookup2 Hh1 => -[].
+      + (* allocate the block in h1 *)
+        iMod (heapUR_alloc_block O1 _ l.1 {[l.2 := v]} with "Hinv1")
+          as "[Hinv1 [Hd Hl']]"; [done|]. iModIntro.
+        rewrite kmap_insert kmap_empty big_sepM_singleton -surjective_pairing.
+        iFrame "Hinv1 Hinv Hl' Hls1".
+        iExists _. iSplitL "Hd Hds1". iApply (big_sepM_insert with "[$]"). admit.
+        rewrite /= map_difference_union_distr.
+        iSplitL "Hls2 Hl".
+        * iApply (big_sepM_union_2 with "[Hl] Hls2").
+          admit.
+        * admit.
+  Abort.
+
+  Lemma heapUR_trade_dom h p d:
+    heapUR_trader W1 W2 O1 O2 -∗
+    ⌈heapUR_inv O2 h @ W2⌉ -∗
+    ⌈p ↪[O2] d @ W2⌉ ==∗⌈W1⌉
+    heapUR_trader W1 W2 O1 O2 ∗
+    ⌈heapUR_inv O2 h @ W2⌉ ∗
+    ⌈p ↪[O1] d @ W1⌉.
+  Proof.
+    iIntros "(%h1 & %ls & %ds & Hinv1 & Hls1 & Hds1 & Hls2 & Hds2) Hinv2 Hd".
+    destruct (decide (p ∈ h_provs h1)).
+    - destruct (ds !! p) as [d'|] eqn:Hds.
+      + iDestruct (big_sepM_insert_acc with "Hds1") as "[??]"; [done|].
+
+ (* deallocate all locations in p that are in ls (works because we have the pointstos for them),
+           allocate all locations with 0 that are in g,
+           the locations in h_heap h1 can stay unchanged since we have the pointsto *)
+        admit.
+      + iDestruct (big_sepM_lookup_acc with "Hds2") as "[??]".
+        { apply lookup_difference_Some. split; [|done]. by apply h_block_doms_lookup_Some. }
+        iDestruct (heapUR_dom_excl (PROP:=PROP2) with "Hd [$]") as %[].
+    - iMod (heapUR_alloc_block O1 _ p (gset_to_gmap (ValNum 0%Z) d) with "Hinv1") as "[Hinv1 [Hd' Hls']]"; [done|].
+      iModIntro. rewrite dom_gset_to_gmap weak_embed_big_sepM. iFrame "Hinv1 Hinv2 Hd' Hds1".
+      iExists _. iSplitL "Hls1 Hls'"; [iApply (big_sepM_union_2 with "Hls1 Hls'")|]. iSplitL "Hls2".
+      + rewrite /= map_difference_union_distr (map_difference_empty_dom (gmap_uncurry _)) ?left_id_L.
+        * rewrite -map_difference_difference (map_difference_disj_id (_ ∖ _)) //.
+          apply map_disjoint_spec => ??? /lookup_difference_Some[/lookup_heap_Some_elem_of_h_provs? ?] /lookup_kmap_Some. naive_solver.
+        * move => [??] /elem_of_dom [?]. rewrite lookup_gmap_uncurry. move => /bind_Some[? [/lookup_singleton_Some[??] Hl]]. simplify_eq/=.
+          rewrite dom_union_L. apply elem_of_union. right. apply elem_of_dom. eexists _. apply/lookup_kmap_Some. naive_solver.
+      + admit.
+  Abort.
+
+  Lemma heapUR_trade_ptsto_big h m:
+    heapUR_trader W1 W2 O1 O2 -∗
+    ⌈heapUR_inv O2 h @ W2⌉ -∗
+    ⌈[∗ map] l↦v∈m, l ↦[O2] v @ W2⌉ ==∗⌈W1⌉
+    heapUR_trader W1 W2 O1 O2 ∗
+    ⌈heapUR_inv O2 h @ W2⌉ ∗
+    ⌈[∗ map] l↦v∈m, l ↦[O1] v @ W1⌉.
+  Proof using BiAffine0.
+    iIntros "Ht Hinv Hl".
+    iInduction m as [|] "IH" using map_ind.
+    { iModIntro. iFrame. iModIntro. done. }
+    rewrite !big_sepM_insert //. iDestruct "Hl" as "[??]".
+    iMod (heapUR_trade_ptsto with "[$] [$] [$]") as "[? [? $]]".
+    iApply ("IH" with "[$] [$] [$]").
+  Qed.
+
+  Lemma heapUR_trade_block h p b:
+    heapUR_trader W1 W2 O1 O2 -∗
+    ⌈heapUR_inv O2 h @ W2⌉ -∗
+    ⌈p ↦∗[O2] b @ W2⌉ ==∗⌈W1⌉
+    heapUR_trader W1 W2 O1 O2 ∗
+    ⌈heapUR_inv O2 h @ W2⌉ ∗
+    ⌈p ↦∗[O1] b @ W1⌉.
+  Proof using BiAffine0.
+    iIntros "Ht Hinv [Hd Hl]".
+    iMod (heapUR_trade_dom with "[$] [$] [$]") as "[? [? $]]".
+    by iMod (heapUR_trade_ptsto_big with "[$] [$] [$]") as "$".
+  Qed.
+
+  Lemma heapUR_trade_block_big h bs:
+    heapUR_trader W1 W2 O1 O2 -∗
+    ⌈heapUR_inv O2 h @ W2⌉ -∗
+    ⌈[∗ map] p↦b∈ bs, p ↦∗[O2] b @ W2⌉ ==∗⌈W1⌉
+    heapUR_trader W1 W2 O1 O2 ∗
+    ⌈heapUR_inv O2 h @ W2⌉ ∗
+    ⌈[∗ map] p↦b∈ bs, p ↦∗[O1] b @ W1⌉.
+  Proof using BiAffine0.
+    iIntros "Ht Hinv Hbs".
+  Abort.
+End trader.
+*)
+
+Global Typeclasses Opaque heapUR_trader.
+Global Opaque heapUR_trader.
