dimsum_examples/rec_heap_inj_vertical.v
@@ -1,0 +1,902 @@
+From dimsum.examples Require Import rec_heap_inj.
+From dimsum.core.iris Require Import weak_embed sat.
+
+Set Default Proof Using "Type".
+
+(** ** Definitions for combining and splitting injections *)
+(** abbreviation: rhiv: rec_heap_inj_vertical *)
+(** inj: souce -> impl, injb: source -> middle, inja: middle -> impl *)
+
+(** [rhiv_combine inja injb] combines the small injections [inja] and
+[injb] into a large injection *)
+Definition rhiv_combine (inja injb : gmap prov loc) : gmap prov loc :=
+  omap (λ l, (λ li, li +ₗ l.2) <$> inja !! l.1) injb.
+
+(** [rhiv_core_b inja injb] computes the part of [injb] that is also
+used by the large injection *)
+Definition rhiv_core_b (inja injb : gmap prov loc) : gmap prov loc :=
+  filter (λ x, is_Some (inja !! x.2.1)) injb.
+
+(** [rhiv_core_b inja injb] computes the part of [inja] that is also
+used by the large injection *)
+Definition rhiv_core_a (inja injb : gmap prov loc) : gmap prov loc :=
+  filter (λ x, x.1 ∈ set_map (D:=gset _) fst (map_img (SA:=gset loc) injb)) inja.
+
+(** [rhiv_proj_b inj inja injb X] projects a new b injection [injb'] injection
+from the large injection [inj]. It preserves the previous [injb] and
+allocates new provenances in the middle from outside [X]. *)
+Definition rhiv_proj_b (inj inja injb : gmap prov loc) (X : gset prov) : gmap prov loc :=
+  injb ∪ ((λ p, (p, 0%Z)) <$> fresh_map (dom inj) X).
+
+(** [rhiv_proj_a inj inja injb X] projects a new a injection [inja'] injection
+from the large injection [inj]. It preserves the previous [inja] and
+allocates new provenances in the middle from outside [X]. *)
+Definition rhiv_proj_a (inj inja injb : gmap prov loc) (X : gset prov) : gmap prov loc :=
+  inja ∪ kmap (λ p, fresh_map (dom inj) X !!! p) (inj ∖ injb).
+
+(** [rhiv_residual] is what is left in the middle heap after the
+small injections are converted to large injection. *)
+Definition rhiv_residual {Σ} `{!satG Σ heap_injUR} (γa γb : gname) (l : loc) : iProp Σ :=
+  ∃ b, ⌜l.2 = 0⌝ ∗ ⌈l.1 ↦∗hi b @ sat γb⌉ ∗ ⌈l.1 ↦∗hs b @ sat γa⌉.
+
+(** *** Lookup lemmas *)
+Lemma rhiv_combine_lookup_Some inja injb ps li0:
+  rhiv_combine inja injb !! ps = Some li0 ↔
+   ∃ l li', injb !! ps = Some l ∧ inja !! l.1 = Some li' ∧ li0 = li' +ₗ l.2.
+Proof.
+  rewrite /rhiv_combine lookup_omap_Some. f_equiv => ? /=.
+  rewrite fmap_Some. naive_solver.
+Qed.
+
+Lemma rhiv_core_b_lookup_Some inja injb p l :
+  rhiv_core_b inja injb !! p = Some l ↔
+   injb !! p = Some l ∧ is_Some (inja !! l.1).
+Proof. by rewrite /rhiv_core_b map_lookup_filter_Some. Qed.
+
+Lemma rhiv_core_b_lookup_None inja injb p :
+  rhiv_core_b inja injb !! p = None ↔
+   (∀ l, injb !! p = Some l → inja !! l.1 = None).
+Proof.
+  rewrite eq_None_not_Some /is_Some.
+  setoid_rewrite rhiv_core_b_lookup_Some. split.
+  2: rewrite /is_Some; naive_solver.
+  move => Hl l ?. apply eq_None_not_Some. naive_solver.
+Qed.
+
+Lemma rhiv_core_a_lookup_Some inja injb p l :
+  rhiv_core_a inja injb !! p = Some l ↔
+   inja !! p = Some l ∧ ∃ ps lm, injb !! ps = Some lm ∧ lm.1 = p.
+Proof.
+  rewrite /rhiv_core_a map_lookup_filter_Some /=.
+  rewrite elem_of_map. setoid_rewrite elem_of_map_img.
+  naive_solver.
+Qed.
+
+Lemma rhiv_proj_b_lookup_Some inj inja injb X p (l : loc) :
+  rhiv_proj_b inj inja injb X !! p = Some l ↔
+   injb !! p = Some l ∨ injb !! p = None ∧
+     fresh_map (dom inj) X !! p = Some l.1 ∧ l.2 = 0.
+Proof.
+  rewrite /rhiv_proj_b lookup_union_Some_raw. do 2 f_equiv.
+  rewrite lookup_fmap_Some. destruct l; naive_solver.
+Qed.
+
+Lemma rhiv_proj_a_lookup_Some inj inja injb X p (l : loc) :
+  rhiv_proj_a inj inja injb X !! p = Some l ↔
+   inja !! p = Some l ∨ inja !! p = None ∧
+     ∃ ps, inj !! ps = Some l ∧ injb !! ps = None ∧ fresh_map (dom inj) X !! ps = Some p.
+Proof.
+  rewrite /rhiv_proj_a lookup_union_Some_raw. do 2 f_equiv.
+  rewrite lookup_kmap_Some_strong. 2: {
+    move => i j [?/lookup_difference_Some[??]] [?/lookup_difference_Some[??]].
+    rewrite !lookup_total_alt.
+    destruct (fresh_map (dom inj) X !! i) eqn:Heq. 2: {
+      move: Heq => /fresh_map_lookup_None/not_elem_of_dom. naive_solver. }
+    destruct (fresh_map (dom inj) X !! j) eqn:Heq2. 2: {
+      move: Heq2 => /fresh_map_lookup_None/not_elem_of_dom. naive_solver. }
+    move => ?. simplify_eq/=. apply (fresh_map_bij _ _ _ _ _ Heq Heq2).
+  }
+  f_equiv => ?. rewrite lookup_difference_Some.
+  split => -[??]; destruct!; split!; subst.
+  - apply lookup_lookup_total. by apply fresh_map_lookup_is_Some, elem_of_dom.
+  - by erewrite lookup_total_correct.
+Qed.
+
+
+(** *** Lemmas about the definitions  *)
+(** [rhiv_combine] is monotonic. *)
+Lemma rhiv_combine_subseteq inja injb inja' injb':
+  inja ⊆ inja' →
+  injb ⊆ injb' →
+  rhiv_combine inja injb ⊆ rhiv_combine inja' injb'.
+Proof.
+  move => Hsuba Hsubb. apply map_subseteq_spec => ??.
+  rewrite !rhiv_combine_lookup_Some.
+  move => [? [? [/(lookup_weaken _ _ _ _)/(_ Hsubb)? [/(lookup_weaken _ _ _ _)/(_ Hsuba) ??]]]].
+  naive_solver.
+Qed.
+
+(** [rhiv_core_a] is smaller than [inja] *)
+Lemma rhiv_core_a_subseteq inja injb :
+  rhiv_core_a inja injb ⊆ inja.
+Proof. apply map_subseteq_spec => ?? /rhiv_core_a_lookup_Some. naive_solver. Qed.
+
+(** [rhiv_core_b] is smaller than [inja] *)
+Lemma rhiv_core_b_subseteq inja injb :
+  rhiv_core_b inja injb ⊆ injb.
+Proof. apply map_subseteq_spec => ?? /rhiv_core_b_lookup_Some. naive_solver. Qed.
+
+(** [rhiv_proj_a] is bigger than [inja] *)
+Lemma rhiv_proj_a_subseteq inj inja injb X :
+  inja ⊆ rhiv_proj_a inj inja injb X.
+Proof. apply map_union_subseteq_l. Qed.
+
+(** [rhiv_proj_b] is bigger than [injb] *)
+Lemma rhiv_proj_b_subseteq inj inja injb X :
+  injb ⊆ rhiv_proj_b inj inja injb X.
+Proof. apply map_union_subseteq_l. Qed.
+
+(** We can convert the new large injection [inj] as a combination of
+the projections. *)
+Lemma rhiv_combine_proj inj inja injb X :
+  (** inj only grew *)
+  rhiv_combine inja injb ⊆ inj →
+  (** inj does have provs that are already in injb (except for those in the core) *)
+  (** We do not need a similar assumption for inja since it is fine to map multiple
+    source provs to the same target *)
+  inj ##ₘ injb ∖ rhiv_core_b inja injb →
+  (** newly allocated provs must be disjoint from the existing ones in inja and injb *)
+  dom inja ⊆ X →
+  map_img (fst <$> injb) ⊆ X →
+  inj = rhiv_combine (rhiv_proj_a inj inja injb X) (rhiv_proj_b inj inja injb X).
+Proof.
+  move => Hsub Hdisj HXa HXb.
+  apply map_eq => p. apply option_eq => li.
+  rewrite rhiv_combine_lookup_Some.
+  setoid_rewrite rhiv_proj_a_lookup_Some.
+  setoid_rewrite rhiv_proj_b_lookup_Some.
+  split => ?.
+  - exploit @map_disjoint_Some_l; [done..|].
+    move => /lookup_difference_None[?|[?/rhiv_core_b_lookup_Some[?[??]]]].
+    + have [??]: is_Some (fresh_map (dom inj) X !! p) by apply fresh_map_lookup_is_Some, elem_of_dom.
+      eexists (_, _), _. split!. 2: by rewrite offset_loc_0. right.
+      split! => //. exploit @fresh_map_lookup_Some; [done|]. move => [_ Hnotin].
+      apply eq_None_not_Some => -[?]. contradict Hnotin. apply HXa.
+      by apply elem_of_dom.
+    + move: Hsub =>/map_subseteq_spec Hsub.
+      exploit Hsub. { apply rhiv_combine_lookup_Some. naive_solver. }
+      naive_solver.
+  - destruct!.
+    + move: Hsub =>/map_subseteq_spec Hsub. apply Hsub.
+      apply rhiv_combine_lookup_Some. naive_solver.
+    + exploit @fresh_map_lookup_Some; [done|]. move => [_ Hnotin].
+      contradict Hnotin. apply HXa. by apply elem_of_dom.
+    + exploit @fresh_map_lookup_Some; [done|]. move => [_ Hnotin].
+      contradict Hnotin. apply HXb, elem_of_map_img. eexists _.
+      apply lookup_fmap_Some. naive_solver.
+    + have ? : p = ps by apply: fresh_map_bij. rewrite H5 offset_loc_0. naive_solver.
+Qed.
+
+(** The core of a only grows. *)
+Lemma rhiv_core_a_proj_subseteq inja injb inj X :
+  rhiv_core_a inja injb ⊆ rhiv_core_a (rhiv_proj_a inj inja injb X) (rhiv_proj_b inj inja injb X).
+Proof.
+  apply map_subseteq_spec => ?? /rhiv_core_a_lookup_Some [? [? [? [??]]]].
+  apply rhiv_core_a_lookup_Some. split.
+  - apply rhiv_proj_a_lookup_Some. naive_solver.
+  - eexists _, _. split; [|done]. apply rhiv_proj_b_lookup_Some. naive_solver.
+Qed.
+
+
+(** The core of b only grows. *)
+Lemma rhiv_core_b_proj_subseteq inja injb inj X :
+  rhiv_core_b inja injb ⊆ rhiv_core_b (rhiv_proj_a inj inja injb X) (rhiv_proj_b inj inja injb X).
+Proof.
+  apply map_subseteq_spec => ?? /rhiv_core_b_lookup_Some [? [??]].
+  apply rhiv_core_b_lookup_Some. split.
+  - apply rhiv_proj_b_lookup_Some. naive_solver.
+  - eexists _. apply rhiv_proj_a_lookup_Some. naive_solver.
+Qed.
+
+
+(** This lemma allows us to build the new a injection [inja'] by
+replacing the core of [inja]. (Technically, we only need the right to
+left inclusion.) *)
+Lemma rhiv_recombine_a inja injb inja' injb' inj' X :
+  inja' = rhiv_proj_a inj' inja injb X →
+  injb' = rhiv_proj_b inj' inja injb X →
+  (inja ∖ rhiv_core_a inja injb ∪ rhiv_core_a inja' injb') = inja'.
+Proof.
+  move => -> ->.
+  apply map_eq => pm. apply option_eq => li.
+  rewrite lookup_union_Some_raw lookup_difference_Some lookup_difference_None.
+  split.
+  - move => [[??]| [? /rhiv_core_a_lookup_Some [??]]] //.
+    apply: lookup_weaken; [done|]. apply rhiv_proj_a_subseteq.
+  - move => /rhiv_proj_a_lookup_Some[?|[?[?[?[??]]]]].
+    + destruct (rhiv_core_a inja injb !! pm) eqn:Heq; [|naive_solver]. split!.
+      apply: lookup_weaken. 2: apply rhiv_core_a_proj_subseteq.
+      move: (Heq) => /rhiv_core_a_lookup_Some. naive_solver.
+    + split!. by left. apply rhiv_core_a_lookup_Some. split.
+      * apply rhiv_proj_a_lookup_Some. naive_solver.
+      * eexists _, (_, _). split!. apply rhiv_proj_b_lookup_Some. by right.
+Qed.
+
+(** This lemma allows us to build the new a injection [injb'] by
+replacing the core of [injb]. (Technically, we only need the right to
+left inclusion.) *)
+Lemma rhiv_recombine_b inja injb inja' injb' inj' X :
+  inja' = rhiv_proj_a inj' inja injb X →
+  injb' = rhiv_proj_b inj' inja injb X →
+  dom inja ⊆ X →
+  (injb ∖ rhiv_core_b inja injb ∪ rhiv_core_b inja' injb') = injb'.
+Proof.
+  move => -> -> HXa.
+  apply map_eq => ps. apply option_eq => lm.
+  rewrite lookup_union_Some_raw lookup_difference_Some lookup_difference_None.
+  rewrite rhiv_core_b_lookup_None rhiv_core_b_lookup_Some.
+  split.
+  - move => [[??]|[?[??]]] //. apply: lookup_weaken; [done|].
+    apply rhiv_proj_b_subseteq.
+  - move => /rhiv_proj_b_lookup_Some[?|[?[??]]].
+    + destruct (inja !! lm.1) eqn:?.
+      * right. split!. { eexists _. apply rhiv_core_b_lookup_Some. naive_solver. }
+        { apply rhiv_proj_b_lookup_Some. naive_solver. }
+        eexists _. apply rhiv_proj_a_lookup_Some. by left.
+      * left. split!. move => ??. unfold loc in *. by simplify_eq.
+    + split!. by left.
+      * apply rhiv_proj_b_lookup_Some. naive_solver.
+      * exploit @fresh_map_lookup_Some; [done|].
+        move => [/elem_of_dom[??] Hnotin]. eexists _.
+        apply rhiv_proj_a_lookup_Some. right. split! => //.
+        apply eq_None_not_Some => -[?]. contradict Hnotin. apply HXa.
+        by apply elem_of_dom.
+Qed.
+
+(** [rhiv_combine_to_b] allows us to express [rhiv_combine] in terms of [rhiv_core_b]. *)
+Lemma rhiv_combine_to_b inja injb :
+  rhiv_combine inja injb = (λ l, inja !!! l.1 +ₗ l.2) <$> rhiv_core_b inja injb.
+Proof.
+  apply map_eq => ?. apply option_eq => ?. rewrite rhiv_combine_lookup_Some.
+  rewrite lookup_fmap_Some. setoid_rewrite rhiv_core_b_lookup_Some.
+  rewrite /is_Some. split => ?; destruct!/=; split!.
+  - by erewrite lookup_total_correct.
+  - by erewrite lookup_total_correct.
+Qed.
+
+(** provs in the new core that are not in the old core are fresh *)
+Lemma rhiv_core_b_proj_fresh inj inja injb X p (l : loc):
+  map_img (fst <$> injb) ⊆ X →
+  (rhiv_core_b (rhiv_proj_a inj inja injb X) (rhiv_proj_b inj inja injb X) ∖
+     rhiv_core_b inja injb) !! p = Some l →
+  fresh_map (dom inj) X !! p = Some l.1 ∧ l.2 = 0.
+Proof.
+  move => HXb /lookup_difference_Some[/rhiv_core_b_lookup_Some[/rhiv_proj_b_lookup_Some Horb [? /rhiv_proj_a_lookup_Some Hora]] /rhiv_core_b_lookup_None?].
+  destruct Horb as [|[?[??]]]; [|done].
+  destruct Hora as [|[? [?[? [??]]]]]; [naive_solver|].
+  exploit @fresh_map_lookup_Some; [done|]. move => [? Hnotin]. contradict Hnotin. apply HXb. apply elem_of_map_img.
+  setoid_rewrite lookup_fmap_Some. naive_solver.
+Qed.
+
+(** Combine the value relation. *)
+Lemma rhiv_combine_val {Σ} `{!satG Σ heap_injUR} inja' injb' γa γb γ vi vm vs:
+  ⌈heap_inj_shared_auth inja' @ sat γa⌉ -∗
+  ⌈heap_inj_shared_auth injb' @ sat γb⌉ -∗
+  ⌈[∗ map] ps↦li0 ∈ rhiv_combine inja' injb', heap_inj_shared ps li0 @ sat γ⌉ -∗
+  ⌈val_in_inj vi vm @ sat γa⌉ -∗
+  ⌈val_in_inj vm vs @ sat γb⌉ -∗
+  ⌈val_in_inj vi vs @ sat γ⌉.
+Proof.
+  iIntros "Ha Hb H Hva Hvb".
+  destruct vi, vm => /=; rewrite ?weak_embed_pure //.
+  all: destruct vs => /=; rewrite ?weak_embed_pure //; iDestruct! => //.
+  iDestruct "Hva" as (??) "Hla".
+  iDestruct "Hvb" as (??) "Hlb". subst => /=.
+  iDestruct (heap_inj_shared_lookup with "Ha [$]") as %?.
+  iDestruct (heap_inj_shared_lookup with "Hb [$]") as %?.
+  iDestruct (big_sepM_lookup (PROP:=uPred heap_injUR) with "[$]") as "?".
+  { apply rhiv_combine_lookup_Some. by split!. }
+  rewrite /loc_in_inj weak_embed_exist.
+  iExists _. iFrame. by rewrite offset_loc_assoc.
+Qed.
+
+Lemma rhiv_combine_val_list {Σ} `{!satG Σ heap_injUR} inja' injb' γa γb γ vi vm vs:
+  ⌈heap_inj_shared_auth inja' @ sat γa⌉ -∗
+  ⌈heap_inj_shared_auth injb' @ sat γb⌉ -∗
+  ⌈[∗ map] ps↦li0 ∈ rhiv_combine inja' injb', heap_inj_shared ps li0 @ sat γ⌉ -∗
+  ⌈[∗ list] v1;v2∈vi;vm, val_in_inj v1 v2 @ sat γa⌉ -∗
+  ⌈[∗ list] v1;v2∈vm;vs, val_in_inj v1 v2 @ sat γb⌉ -∗
+  ⌈[∗ list] v1;v2∈vi;vs, val_in_inj v1 v2 @ sat γ⌉.
+Proof.
+  iIntros "Haa Hab ? Him Hms".
+  iInduction vm as [|] "IH" forall (vi vs). {
+    iDestruct (big_sepL2_nil_inv_r (PROP:=uPred heap_injUR) with "Him") as %->.
+    iDestruct (big_sepL2_nil_inv_l (PROP:=uPred heap_injUR) with "Hms") as %->.
+    simpl. by iPureIntro.
+  }
+  iDestruct (big_sepL2_cons_inv_l (PROP:=uPred heap_injUR) with "Hms") as (?? ->) "[??]".
+  iDestruct (big_sepL2_cons_inv_r (PROP:=uPred heap_injUR) with "Him") as (?? ->) "[??]".
+  simpl.
+  iDestruct (rhiv_combine_val with "Haa Hab [$] [$] [$]") as "#?".
+  iSplit; [done|]. iApply ("IH" with "[$] [$] [$] [$] [$]").
+Qed.
+
+Lemma rhiv_combine_val_map {Σ} `{!satG Σ heap_injUR} `{Countable K} inja' injb' γa γb γ (vi vm vs : gmap K val):
+  ⌈heap_inj_shared_auth inja' @ sat γa⌉ -∗
+  ⌈heap_inj_shared_auth injb' @ sat γb⌉ -∗
+  ⌈[∗ map] ps↦li0 ∈ rhiv_combine inja' injb', heap_inj_shared ps li0 @ sat γ⌉ -∗
+  ⌈[∗ map] v1;v2∈vi;vm, val_in_inj v1 v2 @ sat γa⌉ -∗
+  ⌈[∗ map] v1;v2∈vm;vs, val_in_inj v1 v2 @ sat γb⌉ -∗
+  ⌈[∗ map] v1;v2∈vi;vs, val_in_inj v1 v2 @ sat γ⌉.
+Proof.
+  iIntros "Haa Hab ? Him Hms".
+  iInduction vm as [|] "IH" using map_ind forall (vi vs). {
+    iDestruct (big_sepM2_empty_l (PROP:=uPred heap_injUR) with "Him") as %->.
+    iDestruct (big_sepM2_empty_r (PROP:=uPred heap_injUR) with "Hms") as %->.
+    by rewrite big_sepM2_empty.
+  }
+  iDestruct (big_sepM2_delete_l (PROP:=uPred heap_injUR) with "Hms") as (??) "[??]".
+  { apply lookup_insert. }
+  iDestruct (big_sepM2_delete_r (PROP:=uPred heap_injUR) with "Him") as (??) "[??]".
+  { apply lookup_insert. }
+  rewrite delete_insert //.
+  iDestruct (rhiv_combine_val with "Haa Hab [$] [$] [$]") as "#?".
+  erewrite <-(insert_delete vi) at 2; [|done].
+  erewrite <-(insert_delete vs) at 2; [|done].
+  rewrite big_sepM2_insert; simplify_map_eq => //.
+  iSplit; [done|]. iApply ("IH" with "[$] [$] [$] [$] [$]").
+Qed.
+
+(** Split the value relation. *)
+Lemma rhiv_split_val {Σ} `{!satG Σ heap_injUR} inja' injb' γa γb γ vi vs:
+  ⌈[∗ map] ps↦li0 ∈ inja', heap_inj_shared ps li0 @ sat γa⌉ -∗
+  ⌈[∗ map] ps↦li0 ∈ injb', heap_inj_shared ps li0 @ sat γb⌉ -∗
+  ⌈heap_inj_shared_auth (rhiv_combine inja' injb') @ sat γ⌉ -∗
+
+  ⌈val_in_inj vi vs @ sat γ⌉ -∗
+  ∃ vm, ⌈val_in_inj vi vm @ sat γa⌉ ∗ ⌈val_in_inj vm vs @ sat γb⌉.
+Proof.
+  iIntros "Ha Hb H Hv".
+  destruct vi, vs => /=; rewrite ?weak_embed_pure //; iDestruct!.
+  { iExists (ValNum _) => /=. by iPureIntro. }
+  { iExists (ValBool _) => /=. by iPureIntro. }
+  { iExists (ValFn _) => /=. by iPureIntro. }
+  iDestruct "Hv" as (li ?) "Hl".
+  iDestruct (heap_inj_shared_lookup with "H [$]") as %[lm[li'[?[??]]]]%rhiv_combine_lookup_Some.
+  iDestruct (big_sepM_lookup (PROP:=uPred heap_injUR) with "Ha") as "?"; [done|].
+  iDestruct (big_sepM_lookup (PROP:=uPred heap_injUR) with "Hb") as "?"; [done|].
+  subst. iExists (ValLoc (lm +ₗ l0.2)) => /=. iFrame. iSplit; [|done].
+  unfold loc_in_inj. simpl. iFrame. by rewrite offset_loc_assoc.
+Qed.
+
+Lemma rhiv_split_val_list {Σ} `{!satG Σ heap_injUR} inja' injb' γa γb γ vis vss:
+  ⌈[∗ map] ps↦li0 ∈ inja', heap_inj_shared ps li0 @ sat γa⌉ -∗
+  ⌈[∗ map] ps↦li0 ∈ injb', heap_inj_shared ps li0 @ sat γb⌉ -∗
+  ⌈heap_inj_shared_auth (rhiv_combine inja' injb') @ sat γ⌉ -∗
+
+  ⌈[∗ list] vi;vs∈vis;vss, val_in_inj vi vs @ sat γ⌉ -∗
+  ∃ vms, ⌈[∗ list] vi;vm∈vis;vms, val_in_inj vi vm @ sat γa⌉ ∗
+         ⌈[∗ list] vm;vs∈vms;vss, val_in_inj vm vs @ sat γb⌉.
+Proof.
+  iIntros "Ha Hb H Hv".
+  iInduction vis as [|] "IH" forall (vss). {
+    iDestruct (big_sepL2_nil_inv_l (PROP:=uPred heap_injUR) with "Hv") as %->.
+    iExists []. by simpl.
+  }
+  iDestruct (big_sepL2_cons_inv_l (PROP:=uPred heap_injUR) with "Hv") as (?? ->) "[??]".
+  iDestruct (rhiv_split_val with "Ha Hb [$] [$]") as (?) "#[??]".
+  iDestruct ("IH" with "Ha Hb [$] [$]") as (?) "#[??]".
+  iExists (_::_) => /=. by repeat iSplit.
+Qed.
+
+Lemma rhiv_split_val_map {Σ A} `{!satG Σ heap_injUR} `{Countable A} inja' injb' γa γb γ (vis vss : gmap A val):
+  ⌈[∗ map] ps↦li0 ∈ inja', heap_inj_shared ps li0 @ sat γa⌉ -∗
+  ⌈[∗ map] ps↦li0 ∈ injb', heap_inj_shared ps li0 @ sat γb⌉ -∗
+  ⌈heap_inj_shared_auth (rhiv_combine inja' injb') @ sat γ⌉ -∗
+
+  ⌈[∗ map] vi;vs∈vis;vss, val_in_inj vi vs @ sat γ⌉ -∗
+  ∃ vms, ⌈[∗ map] vi;vm∈vis;vms, val_in_inj vi vm @ sat γa⌉ ∗
+         ⌈[∗ map] vm;vs∈vms;vss, val_in_inj vm vs @ sat γb⌉.
+Proof.
+  iIntros "Ha Hb H Hv".
+  iInduction vis as [|] "IH" using map_ind forall (vss). {
+    iDestruct (big_sepM2_empty_r (PROP:=uPred heap_injUR) with "Hv") as %->.
+    iExists ∅. by rewrite big_sepM2_empty.
+  }
+  iDestruct (big_sepM2_delete_l (PROP:=uPred heap_injUR) with "Hv") as (??) "[??]".
+  { apply lookup_insert. }
+  rewrite delete_insert //.
+  iDestruct (rhiv_split_val with "Ha Hb [$] [$]") as (?) "#[? ?]".
+  iEval (erewrite <-(insert_delete vss); [|done]).
+  iDestruct ("IH" with "[$] [$] [$] [$]") as (vms) "[??]".
+  iExists (<[_:=_]>vms). iSplit.
+  all: by iApply (big_sepM2_insert_2 (PROP:=uPred heap_injUR)); [done|].
+Qed.
+
+(** Allocate the residual for the new provs in the middle heap. *)
+Lemma rhiv_alloc_residual {Σ} `{!satG Σ heap_injUR} (m : gmap prov loc) hm γa γb:
+  map_img (fst <$> m) ## h_provs hm →
+  (∀ i j k, (fst <$> m) !! i = Some k → (fst <$> m) !! j = Some k → i = j) →
+  (∀ i k, m !! i = Some k → k.2 = 0%Z) →
+  (filter is_ProvStatic (map_img (SA:=gset _) (fst <$> m)) = ∅) →
+  ⌈{sat γa}⌉ -∗ ⌈{sat γb}⌉ -∗
+  ⌈heap_inj_inv_s hm @ sat γa⌉ -∗
+  ⌈heap_inj_inv_i hm @ sat γb⌉ ==∗
+  ∃ hm', ([∗ map] li0 ∈ m, rhiv_residual γa γb li0) ∗
+  ⌈{sat γa}⌉ ∗ ⌈{sat γb}⌉ ∗
+  ⌈heap_inj_inv_s hm' @ sat γa⌉ ∗
+  ⌈heap_inj_inv_i hm' @ sat γb⌉ ∗
+  ⌜h_static_provs hm' = h_static_provs hm⌝.
+Proof.
+  iIntros (? Hinj Hm0 Hs) "?? Hinva Hinvb".
+
+  set bs : gmap prov (gmap Z val) := gset_to_gmap ∅ (map_img (fst <$> m)).
+  have ? : dom bs ## h_provs hm by rewrite dom_gset_to_gmap.
+
+  iApply (weak_embed_bupd_intro (sat γa) with "[$]").
+  iMod (heapUR_alloc_blocks own_heap_s _ bs with "Hinva") as "[? Ha]" => //.
+  iIntros "!> ?".
+  iApply (weak_embed_bupd_intro (sat γb) with "[$]").
+  iMod (heapUR_alloc_blocks own_heap_i _ bs with "Hinvb") as "[? Hb]" => //.
+  iIntros "!> ? !>". iFrame. iSplit. 2: {
+    iPureIntro. rewrite h_static_provs_heap_merge h_static_provs_heap_from_blocks.
+    rewrite dom_gset_to_gmap Hs. set_solver.
+  }
+  rewrite !big_sepM_gset_to_gmap !big_sepS_map_img_1 // !big_sepM_fmap.
+  rewrite !weak_embed_big_sepM.
+  iDestruct (big_sepM_sep_2 with "Ha Hb") as "?".
+  iApply (big_sepM_impl with "[$]"). iIntros "!>" (???) "[??]". iExists _. iFrame.
+  iPureIntro. by apply: Hm0.
+Qed.
+
+(** This lemma allows us to integrate the [big_sepM] over
+[rhiv_core_a] into the [big_sepM] for [rhiv_core_b]. This is useful
+since then we only need to do an induction over [rhiv_core_b].
+However, this only holds if [rhiv_core_b] is an injection, i.e. it
+maps different source provenances to different provenances in the
+middle heap. (Otherwise, we would need to reuse the same [Φa l.1 li]
+for multiple elements of [rhiv_core_b]./) *)
+Lemma big_sepM_rhiv_core_a_b_1 {PROP : bi} inja injb (Φa Φb : _ → _ → PROP) `{!BiAffine PROP} `{!BiPureForall PROP}:
+  (** Check that rhiv_core_b is injective *)
+  (∀ p1 p2 l1 l2, ⌜l1.1 = l2.1⌝ -∗ Φb p1 l1 -∗ Φb p2 l2 -∗ False) -∗
+  ([∗ map] p↦l ∈ rhiv_core_a inja injb, Φa p l) -∗
+  ([∗ map] p↦l ∈ rhiv_core_b inja injb, Φb p l) -∗
+  ([∗ map] p↦l ∈ rhiv_core_b inja injb,
+    Φb p l ∗ ∃ li, ⌜rhiv_core_a inja injb !! l.1 = Some li⌝ ∗ Φa l.1 li).
+Proof.
+  iIntros "Hf ? Hb".
+  iAssert ⌜∀ p1 p2 l1 l2, l1.1 = l2.1 → rhiv_core_b inja injb !! p1 = Some l1 → rhiv_core_b inja injb !! p2 = Some l2 → p1 = p2⌝%I as %Himpl. {
+    iIntros (p1 p2 l1 l2 ? ??). destruct (decide (p1 = p2)) => //.
+    rewrite (big_sepM_delete _ (rhiv_core_b _ _)); [|done]. iDestruct "Hb" as "[? Hb]".
+    iDestruct (big_sepM_lookup with "Hb") as "?". { apply lookup_delete_Some. naive_solver. }
+    iDestruct ("Hf" with "[//] [$] [$]") as %[].
+  }
+  iApply big_sepM_sep. iFrame.
+  iApply (big_sepM_impl_rel (λ pa la pb lb, pa = lb.1) with "[$]").
+  move => ?? /rhiv_core_b_lookup_Some[?[??]].
+  split!.
+  - apply rhiv_core_a_lookup_Some. naive_solver.
+  - iIntros "$". iPureIntro. apply rhiv_core_a_lookup_Some. naive_solver.
+  - move => ????. apply: Himpl; [done| |done]. apply rhiv_core_b_lookup_Some. naive_solver.
+Qed.
+
+Lemma big_sepM_rhiv_core_a_b_2 {PROP : bi} inja injb (Φa Φb : _ → _ → PROP) `{!BiAffine PROP}:
+  ([∗ map] p↦l ∈ rhiv_core_b inja injb,
+    Φb p l ∗ ∃ li, ⌜rhiv_core_a inja injb !! l.1 = Some li⌝ ∗ Φa l.1 li) ⊢
+  ([∗ map] p↦l ∈ rhiv_core_a inja injb, Φa p l) ∗
+  ([∗ map] p↦l ∈ rhiv_core_b inja injb, Φb p l).
+Proof.
+  iIntros "Hb".
+  iDestruct (big_sepM_sep with "Hb") as "[$ ?]".
+  iApply (big_sepM_impl_rel (λ pb lb pa la, pa = lb.1) with "[$]").
+  move => ?? /rhiv_core_a_lookup_Some[?[? [? [??]]]].
+  split!.
+  - done.
+  - apply rhiv_core_b_lookup_Some. naive_solver.
+  - iIntros "(%& %Ha & ?)". move: Ha => /rhiv_core_a_lookup_Some[?[?[?[??]]]]. by simplify_eq.
+  - naive_solver.
+Qed.
+
+Lemma big_sepM_rhiv_core_a_b {PROP : bi} inja injb (Φa Φb : _ → _ → PROP) `{!BiAffine PROP} `{!BiPureForall PROP}:
+  (∀ p1 p2 l1 l2, l1.1 = l2.1 → Φb p1 l1 -∗ Φb p2 l2 -∗ False) →
+  ([∗ map] p↦l ∈ rhiv_core_a inja injb, Φa p l) ∗
+  ([∗ map] p↦l ∈ rhiv_core_b inja injb, Φb p l) ⊣⊢
+  ([∗ map] p↦l ∈ rhiv_core_b inja injb,
+    Φb p l ∗ ∃ li, ⌜rhiv_core_a inja injb !! l.1 = Some li⌝ ∗ Φa l.1 li).
+Proof.
+  move => Hf. iSplit.
+  - iIntros "[??]". iApply (big_sepM_rhiv_core_a_b_1 with "[] [$] [$]"). iIntros. by iApply (Hf with "[$] [$]").
+  - iIntros "?". by iApply big_sepM_rhiv_core_a_b_2.
+Qed.
+
+(** Create the large invariant and the residual from the two small invariants. *)
+Lemma rhiv_shared_from_ab {Σ} `{!satG Σ heap_injUR} inja' injb' γa γb γ ha hb hm:
+  heapUR_trader (sat γ) (sat γa) own_heap_i own_heap_i -∗
+  heapUR_trader (sat γ) (sat γb) own_heap_s own_heap_s -∗
+  ⌈heap_inj_inv_i ha @ sat γa⌉ -∗
+  ⌈heap_inj_inv_s hm @ sat γa⌉ -∗
+  ⌈heap_inj_inv_i hm @ sat γb⌉ -∗
+  ⌈heap_inj_inv_s hb @ sat γb⌉ -∗
+  ⌈heap_inj_shared_auth inja' @ sat γa⌉ -∗
+  ⌈heap_inj_shared_auth injb' @ sat γb⌉ -∗
+  ⌈[∗ map] ps↦li0 ∈ rhiv_combine inja' injb', heap_inj_shared ps li0 @ sat γ⌉ -∗
+
+  (** interesting part starts here *)
+  ⌈heap_in_inj_inv (rhiv_core_a inja' injb') [] @ sat γa⌉ -∗
+  ⌈heap_in_inj_inv (rhiv_core_b inja' injb') [] @ sat γb⌉ ==∗⌈sat γ⌉
+  (⌈heap_in_inj_inv (rhiv_combine inja' injb') [] @ sat γ⌉ ∗
+  ([∗ map] ps↦li0 ∈ rhiv_core_b inja' injb', rhiv_residual γa γb li0)) ∗
+  (** interesting part ends here *)
+
+  heapUR_trader (sat γ) (sat γa) own_heap_i own_heap_i ∗
+  heapUR_trader (sat γ) (sat γb) own_heap_s own_heap_s ∗
+  ⌈heap_inj_inv_i ha @ sat γa⌉ ∗
+  ⌈heap_inj_inv_s hm @ sat γa⌉ ∗
+  ⌈heap_inj_inv_i hm @ sat γb⌉ ∗
+  ⌈heap_inj_inv_s hb @ sat γb⌉ ∗
+  ⌈heap_inj_shared_auth inja' @ sat γa⌉ ∗
+  ⌈heap_inj_shared_auth injb' @ sat γb⌉.
+Proof.
+  iIntros "???????? #? ? ?". rewrite /heap_in_inj_inv.
+  have Hempty : ∀ k, k ∈ [] ↔ False by set_solver.
+  setoid_rewrite Hempty. setoid_rewrite bi.False_or.
+  iEval (rewrite rhiv_combine_to_b big_sepM_fmap).
+  rewrite (weak_embed_big_sepM _ _ (rhiv_core_a _ _)).
+  rewrite !(weak_embed_big_sepM _ _ (rhiv_core_b _ _)).
+  iDestruct (big_sepM_rhiv_core_a_b_1 with "[] [$] [$]") as "?".
+  { iIntros (???? ->) "(%&%&?&?&?) (%&%&?&?&?)". iDestruct (heapUR_block_excl own_heap_i with "[$] [$]") as %[]. }
+  rewrite -big_sepM_sep.
+  iMod (big_sepM_impl_weak_bupd_frame with "[$] [] [-]") as "[$ ?]".
+  2: iAccu. 2: by iFrame.
+  iIntros "!>" (???). iIntros "(Hta & Htb & ? & Hma & Hmb & ? & Hsha & Hshb)".
+  iIntros "[(% & % & % & ? & ? & Hvb) Ha]".
+
+  iDestruct "Ha" as (?[??]%rhiv_core_a_lookup_Some) "(% & % & % & ? & ? & Hva)" => //=.
+  iMod (heapUR_trade_block with "Hta [$] [$]") as "[? [??]]".
+  iMod (heapUR_trade_block with "Htb [$] [$]") as "[? [??]]".
+  iDestruct (heapUR_lookup_block (PROP:=uPred heap_injUR) with "Hma [$]") as %?.
+  iDestruct (heapUR_lookup_block (PROP:=uPred heap_injUR) with "Hmb [$]") as %?.
+  simplify_eq.
+  iDestruct (rhiv_combine_val_map with "Hsha Hshb [$] Hva Hvb") as "#?". iFrame.
+  iModIntro. erewrite lookup_total_correct => //. iFrame.
+  repeat iSplit => //. iPureIntro. lia.
+Qed.
+
+(** Create the two small invariants from the large invariant and the residual. *)
+Lemma rec_heap_inj_vertical_shared_to_ab {Σ} `{!satG Σ heap_injUR} inja' injb' γa γb γ ha hb hm:
+  ⌈{sat γa}⌉ -∗ ⌈{sat γb}⌉ -∗
+  heapUR_trader (sat γa) (sat γ) own_heap_i own_heap_i -∗
+  heapUR_trader (sat γb) (sat γ) own_heap_s own_heap_s -∗
+  ⌈heap_inj_inv_i ha @ sat γ⌉ -∗
+  ⌈heap_inj_inv_s hm @ sat γa⌉ -∗
+  ⌈heap_inj_inv_i hm @ sat γb⌉ -∗
+  ⌈heap_inj_inv_s hb @ sat γ⌉ -∗
+  ⌈[∗ map] ps↦li0 ∈ inja', heap_inj_shared ps li0 @ sat γa⌉ -∗
+  ⌈[∗ map] ps↦li0 ∈ injb', heap_inj_shared ps li0 @ sat γb⌉ -∗
+  ⌈heap_inj_shared_auth (rhiv_combine inja' injb') @ sat γ⌉ -∗
+
+  (** interesting part starts here *)
+  ⌈heap_in_inj_inv (rhiv_combine inja' injb') [] @ sat γ⌉ -∗
+  ([∗ map] ps↦li0 ∈ rhiv_core_b inja' injb', rhiv_residual γa γb li0) ==∗
+  ∃ hm',
+  (⌈heap_in_inj_inv (rhiv_core_a inja' injb') [] @ sat γa⌉ ∗
+  ⌈heap_in_inj_inv (rhiv_core_b inja' injb') [] @ sat γb⌉) ∗
+  (** interesting part ends here *)
+
+  ⌈{sat γa}⌉ ∗ ⌈{sat γb}⌉ ∗
+  heapUR_trader (sat γa) (sat γ) own_heap_i own_heap_i ∗
+  heapUR_trader (sat γb) (sat γ) own_heap_s own_heap_s ∗
+  ⌈heap_inj_inv_i ha @ sat γ⌉ ∗
+  ⌈heap_inj_inv_s hm' @ sat γa⌉ ∗
+  ⌈heap_inj_inv_i hm' @ sat γb⌉ ∗
+  ⌈heap_inj_inv_s hb @ sat γ⌉ ∗
+  ⌈heap_inj_shared_auth (rhiv_combine inja' injb') @ sat γ⌉ ∗ ⌜h_static_provs hm' = h_static_provs hm⌝.
+Proof.
+  iIntros "????????#Hsa#Hsb???".
+  rewrite /heap_in_inj_inv.
+  have Hempty : ∀ k, k ∈ [] ↔ False by set_solver.
+  setoid_rewrite Hempty. setoid_rewrite bi.False_or.
+  rewrite {2}rhiv_combine_to_b big_sepM_fmap.
+  setoid_rewrite (weak_embed_big_sepM _ _ (rhiv_core_a _ _)).
+  setoid_rewrite (weak_embed_big_sepM _ _ (rhiv_core_b _ _)).
+  setoid_rewrite big_sepM_rhiv_core_a_b; try apply _.
+  2: { iIntros (???? ->) "(%&%&?&?&?) (%&%&?&?&?)". iDestruct (heapUR_block_excl own_heap_i with "[$] [$]") as %[]. }
+  iDestruct (big_sepM_sep with "[$]") as "Hm".
+  iApply (big_sepM_impl_bupd_ex_frame with "Hm"). 2: by iFrame.
+  iIntros "!>" (???[?[??]]%rhiv_core_b_lookup_Some) "(?&?&Hta&Htb&?&Hinva&Hinvb&?&?&<-) [[%[%[??]]] [%[%[%Htot[Hi[Hs Hv]]]]]]".
+  erewrite lookup_total_correct in Htot |- * => //. simplify_eq/=.
+  iDestruct (rhiv_split_val_map with "Hsa Hsb [$] [$]") as (bm) "#[? ?]". simpl.
+
+  iApply (weak_embed_bupd_intro (sat γa) with "[$]").
+  iDestruct (heapUR_lookup_block_prov own_heap_s with "Hinva [$]") as %?.
+  iMod (heapUR_update_block own_heap_s with "Hinva [$]") as "[? ?]".
+  iMod (heapUR_trade_block with "Hta [$] [$]") as "[? [??]]".
+  iIntros "!> Hγa".
+
+  iApply (weak_embed_bupd_intro (sat γb) with "[$]").
+  iMod (heapUR_update_block own_heap_i with "Hinvb [$]") as "[? ?]".
+  iMod (heapUR_trade_block with "Htb [$] [$]") as "[? [??]]".
+  iIntros "!> Hγb".
+
+  iModIntro. iFrame. iSplit!; repeat iSplit => //.
+  - by rewrite h_static_provs_update_block.
+  - apply rhiv_core_a_lookup_Some. naive_solver.
+  - iPureIntro. lia.
+Qed.
+
+Lemma rec_heap_inj_vertical m hinit `{!VisNoAng m.(m_trans)} :
+  trefines (rec_heap_inj hinit (rec_heap_inj hinit m))
+           (rec_heap_inj hinit m).
+Proof.
+  unshelve apply: mod_prepost_combine_bi.
+  set (Σ := #[satΣ heap_injUR]). have ? : satG Σ heap_injUR by apply _. clearbody Σ.
+  eexists Σ, _, _, _ => γa γb γ.
+  unshelve eexists _.  {
+    exact (λ pl _ _ _,
+      ∃ inja injb inj statics,
+        if pl is Env then
+          (* We only require the subseteq here since it makes the
+          initialization easier. *)
+          ⌜rhiv_combine inja injb ⊆ inj⌝ ∗ ∃ hm,
+          ⌜h_static_provs hm = statics⌝ ∗
+          ⌈[∗ map] ps↦li0∈inj, heap_inj_shared ps li0 @ sat γ⌉ ∗
+          ⌈heap_inj_shared_auth inja @ sat γa⌉ ∗
+          ⌈heap_inj_shared_auth injb @ sat γb⌉ ∗
+          ⌈heap_in_inj_inv (inja ∖ rhiv_core_a inja injb) [] @ sat γa⌉ ∗
+          ⌈heap_in_inj_inv (injb ∖ rhiv_core_b inja injb) [] @ sat γb⌉ ∗
+          ([∗ map] ps↦li0 ∈ rhiv_core_b inja injb, rhiv_residual γa γb li0) ∗
+          ⌈heapUR_inv own_heap_s hm @ sat γa⌉ ∗
+          ⌈heapUR_inv own_heap_i hm @ sat γb⌉ ∗
+          heapUR_trader (sat γa) (sat γ) own_heap_i own_heap_i ∗
+          heapUR_trader (sat γb) (sat γ) own_heap_s own_heap_s ∗
+          (* This proof could be quite a bit simpler without the
+          requirement that the statics stay the same. (It is not used
+          in this proof.) *)
+          ⌈heap_inj_statics statics @ sat γa⌉ ∗
+          ⌈heap_inj_statics statics @ sat γb⌉ ∗
+          ⌈heap_inj_statics statics @ sat γ⌉
+        else
+          ⌜inj = rhiv_combine inja injb⌝ ∗
+          ⌈[∗ map] ps↦li0∈inja, heap_inj_shared ps li0 @ sat γa⌉ ∗
+          ⌈[∗ map] ps↦li0∈injb, heap_inj_shared ps li0 @ sat γb⌉ ∗
+          ⌈heap_inj_shared_auth inj @ sat γ⌉ ∗
+          heapUR_trader (sat γ) (sat γa) own_heap_i own_heap_i ∗
+          heapUR_trader (sat γ) (sat γb) own_heap_s own_heap_s ∗
+          ⌈heap_inj_statics statics @ sat γa⌉ ∗
+          ⌈heap_inj_statics statics @ sat γb⌉ ∗
+          ⌈heap_inj_statics statics @ sat γ⌉
+          )%I. }
+  split_and!.
+  - move => /= e ? h.
+    iIntros "([Hiniti Hinits] & [($&Hinv&[%inj[Hsh ?]]& $ & #?) $] & _)".
+    iDestruct (heapUR_lookup_block_big own_heap_s with "Hinv Hinits") as %Hblocks.
+    set staticbs : gmap prov (gmap Z val) :=
+            gset_to_gmap ∅ (h_static_provs h) ∖ hinit.
+    iExists _, _. iSplit!. {
+      apply: satisfiable_bmono; [apply heap_inj_init|].
+      iIntros "(? & ? & Hinvi & Hinvs)".
+      iMod (heapUR_alloc_blocks with "Hinvi") as "[Hinvi $]"; [set_solver|].
+      iMod (heapUR_alloc_blocks _ _ (hinit ∪ staticbs) with "Hinvs") as "[Hinvs Hbs]"; [set_solver|].
+      iDestruct (big_sepM_union with "Hbs") as "[$ ?]";
+        [apply map_disjoint_difference_r'|].
+      rewrite !right_id. iModIntro. iAccu.
+    } {
+      apply: satisfiable_bmono; [apply heap_inj_init|].
+      iIntros "(? & ? & Hinvi & Hinvs)".
+      iMod (heapUR_alloc_blocks _ _ (hinit ∪ staticbs) with "Hinvi") as "[Hinvi Hbs]"; [set_solver|].
+      iMod (heapUR_alloc_blocks with "Hinvs") as "[Hinvs $]"; [set_solver|].
+      iDestruct (big_sepM_union with "Hbs") as "[$ ?]";
+        [apply map_disjoint_difference_r'|].
+      rewrite !right_id. iModIntro. iAccu.
+    }
+    iIntros "Hγa Hγb Hγ (?&?&Hinvia&?&?) (?&?&?&Hinvsb&?)".
+    iModIntro. iFrame "#∗". iFrame "#".
+    iExists ∅. rewrite /heap_in_inj_inv !big_sepM_empty. iSplit!. {
+      rewrite h_static_provs_heap_from_blocks dom_union_L dom_difference_L.
+      rewrite (comm (R:=(=)) (∪)) difference_union_L.
+      rewrite dom_gset_to_gmap filter_union_L (comm (R:=(=)) (∪)).
+      rewrite subseteq_union_1_L; [set_solver|].
+      rewrite map_subseteq_spec in Hblocks.
+      move => ? /elem_of_filter[?/elem_of_dom[? /Hblocks/h_blocks_lookup_Some[??]]].
+      apply elem_of_filter. split!. by apply elem_of_h_static_provs.
+    }
+    iSplitL "Hinvia Hiniti"; iApply (heapUR_trader_init_blocks with "[$] [$]").
+  - move => /= ??????. iIntros "??? [[Hinv ?] _] (%inja & %injb & %inj & %statics & % & %  & % & ? & Hsha & Hshb & Hinja & Hs)". simplify_eq.
+    iDestruct (big_sepL2_length (PROP:=uPred heap_injUR) with "[$]") as %?.
+    iDestruct "Hs" as "(Hinjb & Hbs & ? & ? & Hta & Htb & #Hsa & #Hsb & #Hs)".
+    iDestruct "Hinv" as "(Hinvi & Hinvs & [%inj' [Hsh Hinj]] & Hs1 & Hs2)".
+    iDestruct (heap_inj_statics_eq with "Hs1 Hs2") as %Heq1.
+    iDestruct (heap_inj_statics_eq with "Hs Hs2") as %Heq2.
+    iDestruct (heap_inj_shared_lookup_big with "Hsh [$]") as %?.
+
+    iAssert ⌜inj' ##ₘ injb ∖ rhiv_core_b inja injb⌝%I as %?. {
+      rewrite map_disjoint_spec.
+      iIntros (?????).
+      iDestruct (heap_in_inj_inv_borrow with "Hinj") as (???) "(?&?&Hp&?)"; [apply not_elem_of_nil|done|].
+      iDestruct (heap_in_inj_inv_borrow with "Hinjb") as (???) "(?&?&?&?)"; [apply not_elem_of_nil|done|].
+      iApply bupd_plainly.
+      iApply (weak_embed_bupd_intro (sat γb) with "[$]").
+      iMod (heapUR_trade_block with "[$] [$] Hp") as "[? [??]]".
+      iDestruct (heapUR_block_excl own_heap_s with "[$] [$]") as %[].
+    }
+
+    (* Technically, h_provs hm should suffice, but it would require more proofs. *)
+    set (X := (dom inja ∪ map_img (fst <$> injb) ∪ h_provs hm)).
+    set (inja' := (rhiv_proj_a inj' inja injb X)).
+    set (injb' := (rhiv_proj_b inj' inja injb X)).
+
+    have -> : inj' = rhiv_combine inja' injb' by
+      apply rhiv_combine_proj; [by etrans |done|set_solver..].
+
+    (** Update the small injections  *)
+    iApply (weak_embed_bupd_intro (sat γb) with "[$]").
+    iMod (heap_inj_shared_alloc_big _ injb' with "Hshb") as "[? #Hshbbig]".
+    { apply rhiv_proj_b_subseteq. }
+    iIntros "!> Hγb". iFrame "Hshbbig".
+
+    iApply (weak_embed_bupd_intro (sat γa) with "[$]").
+    iMod (heap_inj_shared_alloc_big _ inja' with "Hsha") as "[? #Hshabig]".
+    { apply rhiv_proj_a_subseteq. }
+    iIntros "!> Hγa". iFrame "Hshabig".
+
+    (** Update the residual *)
+    iMod (rhiv_alloc_residual (rhiv_core_b inja' injb' ∖ rhiv_core_b inja injb) with "[$] [$] [$] [$]") as (hm') "[Hbs' [Hγa [Hγb[?[?%Heqm]]]]]". {
+      move => ? /elem_of_map_img[? /lookup_fmap_Some[? [? ]]]. subst.
+      move => /rhiv_core_b_proj_fresh[|/(fresh_map_lookup_Some _ _ _ _)]; set_solver.
+    } {
+      move => ??? /lookup_fmap_Some[[??][? /rhiv_core_b_proj_fresh[|??]]]. 1: set_solver.
+      move => /lookup_fmap_Some[[??][? /rhiv_core_b_proj_fresh[|??]]]. 1: set_solver. simplify_eq/=.
+      by apply: fresh_map_bij.
+    } { move => ?? /rhiv_core_b_proj_fresh[|//]. set_solver. } {
+      apply equiv_empty_L. move => ? /elem_of_filter[? /elem_of_map_img[? /lookup_fmap_Some[l [? ]]]]. subst.
+      move => /rhiv_core_b_proj_fresh[//|/fresh_map_is_Block]. 1: set_solver. by destruct l.1.
+    }
+    iDestruct (big_sepM_union_2 with "Hbs Hbs'") as "Hbs".
+    rewrite map_difference_union. 2: { apply rhiv_core_b_proj_subseteq. }
+
+    (** Create the small [heap_in_inj_inv]. *)
+    iMod (rec_heap_inj_vertical_shared_to_ab with "Hγa Hγb Hta Htb [$] [$] [$] [$] [$] [$] [$] [$] [$]") as (?) "([??] & ? & ? & ? & ? & ? & ? & ? & ? & ? & %Heqm')".
+
+    iDestruct (heap_in_inj_inv_combine with "Hinja [$]") as "Hinja".
+    iDestruct (heap_in_inj_inv_combine with "Hinjb [$]") as "Hinjb".
+    erewrite rhiv_recombine_a => //. erewrite rhiv_recombine_b => //.
+    2: set_solver.
+
+    (** Split the val_in_inj for the arguments. *)
+    iDestruct (rhiv_split_val_list with "Hshabig Hshbbig [$] [$]") as (vms) "#[Hv1 ?]".
+    iDestruct (big_sepL2_length (PROP:=uPred heap_injUR) with "Hv1") as %?.
+
+    (** Transfer the traders *)
+    iApply (weak_embed_bupd_intro (sat γb) with "[$]").
+    iMod (heapUR_trader_switch with "[$] [$]") as "[$ ?]".
+    iIntros "!> ?".
+    iApply (weak_embed_bupd_intro (sat γa) with "[$]").
+    iMod (heapUR_trader_switch with "[$] [$]") as "[$ ?]".
+    iIntros "!> ?". iModIntro.
+
+    (** Finish *)
+    iExists vms, _. setoid_rewrite event_set_vals_heap_idemp.
+    rewrite heap_of_event_event_set_vals_heap vals_of_event_event_set_vals_heap //.
+    iFrame "#∗". iSplit!; repeat iSplit => //.
+    + by rewrite Heq1 -Heq2.
+    + by rewrite Heqm' Heqm.
+    + by rewrite Heqm' Heqm.
+    + by rewrite -Heq2.
+
+  - move => /= ????????. iIntros "??? [[Hinva Hva] _] [[Hinvb Hvb] _] (%inja & %injb & %inj & %statics & % & ? & ? & Hsh & Hta & Htb & Hsa & Hsb & #Hs)".
+    iDestruct (big_sepL2_length (PROP:=uPred heap_injUR) with "[$]") as %?.
+    rewrite heap_of_event_event_set_vals_heap event_set_vals_heap_idemp vals_of_event_event_set_vals_heap //.
+    iDestruct "Hinva" as "(Hinvia & Hinvsa & [%inja' [Hsha Hinja]] & Hsa1 & Hsa2)".
+    iDestruct "Hinvb" as "(Hinvib & Hinvsb & [%injb' [Hshb Hinjb]] & Hsb1 & Hsb2)".
+    iDestruct (heap_inj_statics_eq with "Hsa1 Hsa2") as %Heq1.
+    iDestruct (heap_inj_statics_eq with "Hsa Hsa1") as %?.
+    iDestruct (heap_inj_statics_eq with "Hsb1 Hsb2") as %Heq2.
+    iDestruct (heap_inj_statics_eq with "Hsb Hsb1") as %?.
+    iFrame "Hsa Hsb Hs".
+    iDestruct (heap_inj_shared_lookup_big with "Hsha [$]") as %?.
+    iDestruct (heap_inj_shared_lookup_big with "Hshb [$]") as %?.
+
+    (** Update the large injection *)
+    iApply (weak_embed_bupd_intro (sat γ) with "[$]").
+    iMod (heap_inj_shared_alloc_big _ (rhiv_combine inja' injb') with "Hsh") as "[? #Hshbig]".
+    { subst. by apply rhiv_combine_subseteq. }
+    iIntros "!> ?". iFrame "Hshbig".
+
+    (** Split the small invariants *)
+    iDestruct (heap_in_inj_inv_split (rhiv_core_a inja' injb') with "Hinja") as "[? Hinja]"; [apply rhiv_core_a_subseteq|].
+    iDestruct (heap_in_inj_inv_split (rhiv_core_b inja' injb') with "Hinjb") as "[? Hinjb]"; [apply rhiv_core_b_subseteq|].
+    iFrame "Hinja Hinjb".
+
+    (** Combine the small invariants to get the large invariant. *)
+    iApply (weak_embed_bupd_intro (sat γ) with "[$]").
+    iMod (rhiv_shared_from_ab with "[$] [$] [$] [$] [$] [$] [$] [$] [$] [$] [$]") as "[[??][?[?[? [? [? [? [Hsha Hshb]]]]]]]]".
+
+    (** Combine the val_in_inj for the arguments. *)
+    iDestruct (rhiv_combine_val_list with "Hsha Hshb [$] [$] [$]") as "#?".
+
+    (** Transfer the traders *)
+    iMod (heapUR_trader_switch with "[$] [$]") as "[$ $]".
+    iMod (heapUR_trader_switch with "[$] [$]") as "[$ ?]".
+    iIntros "!> ?". iModIntro.
+
+    (** Finish *)
+    iExists _, _. iFrame. iSplit!.
+    repeat iSplit.
+    + by subst.
+    + subst. by rewrite -Heq2 -Heq1.
+    + done.
+Qed.
+
+(*
+For the following definition of the sharing invariant, it is impossible to prove
+vertical compositionality:
+
+Definition heap_in_inj_inv (inj : gmap prov loc) (rem : list prov) :
+  uPred heap_injUR :=
+    [∗ map] ps↦li0∈inj, ⌜ps ∈ rem⌝ ∨
+      ∃ b, heap_inj_block_s ps b ∗
+      [∗ map] o↦vs∈b, ∃ vi, (li0 +ₗ o) ↦hi vi ∗ val_in_inj vi vs.
+
+This is because of the following situation:
+
+In the two wrappers, we have two blocks that are mapped to two different blocks
+in the first wrapper and to one block in the second wrapper:
+
+---  ---
+| |  | |
+---  ---
+| |  | |
+--------
+
+From the perspective of the single wrapper, the middle blocks disappear, so it looks
+like this:
+---  ---
+| |  | |
+| |  | |
+| |  | |
+--------
+
+Now the outer code can move locations from the second to the first block.
+This works since it does not need the dom in the target for this, resulting in a
+picture like the following:
+
+----  --
+|  |  ||
+|  |  ||
+|  |  ||
+--------
+
+However, we cannot backtranslate this picture to the two wrappers, since we do not
+have the dom for the provenances in the middle and in fact the code in the middle
+might rely on the fact that the dom of the provenances in the middle does not change.
+
+---  ---
+| |  | |
+---  ---
+|  |  ||
+--------
+
+So one could prove false from the vertical composition with suitable modules.
+
+One idea to get an injection wrapper that is vertically composable is to not put
+the full dom of the source into the sharing invariant, but only 1/2 fraction.
+This would mean that each module can only change the size of blocks that it allocated
+itself. This seems like a reasonable solution, but the resulting wrapper would be
+incomparable to the existing bijection wrapper. In the vertical composition proof,
+one would make sure that one has all doms for the middle heap for the provenances
+that were shared by the environment. This would require some looking into the trader
+to make sure that one never trades a full dom that belongs to the inner module.
+
+The definition of the invariant could look like this:
+
+Definition heap_in_inj_inv (inj : gmap prov loc) (rem : list prov) :
+  uPred heap_injUR :=
+    [∗ map] ps↦li0∈inj, ⌜ps ∈ rem⌝ ∨
+      ∃ d, heap_inj_dom_s ps (1/2) d ∗
+      [∗ map] o∈d, ∃ vi vs, (li0 +ₗ o) ↦hi vi ∗ (p, o) ↦hs vs ∗ val_in_inj vi vs.
+
+An alternative idea is to add some more ghost state that ensure that shared blocks
+can only shrink, but not grow. This would allow deallocation by other modules, while
+preventing the problematic situation from above but otherwise restrict everything
+quite a bit more. Also setting up the extra ghost state would be more tricky.
+*)
